@prefix : <https://w3id.org/won/ext/persona#> .
@prefix dc: <http://purl.org/dc/elements/1.1/> .
@prefix owl: <http://www.w3.org/2002/07/owl#> .
@prefix rdf: <http://www.w3.org/1999/02/22-rdf-syntax-ns#> .
@prefix won: <https://w3id.org/won/core#> .
@prefix xml: <http://www.w3.org/XML/1998/namespace> .
@prefix xsd: <http://www.w3.org/2001/XMLSchema#> .
@prefix rdfs: <http://www.w3.org/2000/01/rdf-schema#> .
@prefix vann: <http://purl.org/vocab/vann/> .
@prefix dcterms: <http://purl.org/dc/terms/> .
@base <https://w3id.org/won/ext/persona> .

<https://w3id.org/won/ext/persona> rdf:type owl:Ontology ;
                                 owl:versionIRI <https://w3id.org/won/ext/persona/1.0> ;
                                 owl:imports <https://w3id.org/won/core> ;
                                 dc:abstract "This ontology contains the definition of the *InterestSocket* the *InterestOfSocket* the *ExpertiseSocket* and the *ExpertiseOfSocket*, the *interest* the *interestOf* the *expertise* and the *expertOf* properties. These express control relationships in WoN. The Atoms with expertise/interest in other atoms represent agents (users or programs) and can themselves not be interests/expertises of other atoms."@en ;
                                 dc:creator "Fabian Suda" ;
                                 dc:date "2021-02-02"^^xsd:date ;
                                 dc:title "Web of Needs Persona Extension" ;
                                 dcterms:license <https://creativecommons.org/licenses/by/4.0/> ;
                                 vann:preferredNamespacePrefix "wx-persona" .

#################################################################
#    Annotation properties
#################################################################

###  http://purl.org/dc/elements/1.1/abstract
dc:abstract rdf:type owl:AnnotationProperty .


###  http://purl.org/dc/elements/1.1/creator
dc:creator rdf:type owl:AnnotationProperty .


###  http://purl.org/dc/elements/1.1/date
dc:date rdf:type owl:AnnotationProperty .


###  http://purl.org/dc/elements/1.1/description
dc:description rdf:type owl:AnnotationProperty .


###  http://purl.org/dc/elements/1.1/title
dc:title rdf:type owl:AnnotationProperty .


###  http://purl.org/dc/terms/license
dcterms:license rdf:type owl:AnnotationProperty .


###  http://purl.org/vocab/vann/preferredNamespacePrefix
vann:preferredNamespacePrefix rdf:type owl:AnnotationProperty .


###  http://www.w3.org/2000/01/rdf-schema#labels
rdfs:labels rdf:type owl:AnnotationProperty .


#################################################################
#    Classes
#################################################################

###  https://w3id.org/won/ext/persona#Interest
:Interest rdf:type owl:Class ;
          rdfs:comment "Announce an interest in something, such as a hobby."@en ;
          rdfs:label "Interest" .

###  https://w3id.org/won/ext/persona#Expertise
:Expertise rdf:type owl:Class ;
          rdfs:comment "Announce an expertise in something, such as a technology or framework."@en ;
          rdfs:label "Expertise" .

#################################################################
#    Object Properties
#################################################################

###  https://w3id.org/won/ext/persona#interestOf
:interestOf rdf:type owl:ObjectProperty ;
        rdfs:domain won:Atom ;
        rdfs:range won:Atom ;
        owl:propertyDisjointWith :interest .


###  https://w3id.org/won/ext/persona#interest
:interest rdf:type owl:ObjectProperty ;
       rdfs:domain won:Atom ;
       rdfs:range won:Atom .

###  https://w3id.org/won/ext/persona#expertiseOf
:expertiseOf rdf:type owl:ObjectProperty ;
        rdfs:domain won:Atom ;
        rdfs:range won:Atom ;
        owl:propertyDisjointWith :expertise .


###  https://w3id.org/won/ext/persona#expertise
:expertise rdf:type owl:ObjectProperty ;
       rdfs:domain won:Atom ;
       rdfs:range won:Atom .

#################################################################
#    Individuals
#################################################################

###  https://w3id.org/won/ext/persona#InterestOfSocket
:InterestOfSocket rdf:type owl:NamedIndividual ,
                         won:SocketDefinition ;
                won:compatibleSocketDefinition :InterestSocket ;
                won:derivesAtomProperty :interestOf ;
                won:autoOpen "false"^^xsd:boolean ;
                won:socketCapacity 1 ;
                rdfs:comment "An Atom uses a Socket with this configuration to identify an interest of the Persona Atom that it is connected to."@en ;
                rdfs:label "InterestOfSocket" .


###  https://w3id.org/won/ext/persona#InterestSocket
:InterestSocket rdf:type owl:NamedIndividual ,
                       won:SocketDefinition ;
              won:compatibleSocketDefinition :InterestOfSocket ;
              won:derivesAtomProperty :interest ;
              won:autoOpen "false"^^xsd:boolean ;
              rdfs:comment "A Persona Atom uses a Socket with this configuration to represent Interests."@en ;
              rdfs:label "InterestSocket" .

###  https://w3id.org/won/ext/persona#InterestOfSocket
:ExpertiseOfSocket rdf:type owl:NamedIndividual ,
                         won:SocketDefinition ;
                won:compatibleSocketDefinition :ExpertiseSocket ;
                won:derivesAtomProperty :expertiseOf ;
                won:autoOpen "false"^^xsd:boolean ;
                won:socketCapacity 1 ;
                rdfs:comment "An Atom uses a Socket with this configuration to identify an expertise of the Persona Atom that it is connected to"@en ;
                rdfs:label "ExpertiseOfSocket" .


###  https://w3id.org/won/ext/persona#InterestSocket
:ExpertiseSocket rdf:type owl:NamedIndividual ,
                       won:SocketDefinition ;
              won:compatibleSocketDefinition :ExpertiseOfSocket ;
              won:derivesAtomProperty :expertise ;
              won:autoOpen "false"^^xsd:boolean ;
              rdfs:comment "A Persona Atom uses a Socket with this configuration to represent Expertises."@en ;
              rdfs:label "ExpertiseSocket" .

#################################################################
#    Annotations
#################################################################

:interestOf rdfs:label "interestOf" ;
        rdfs:comment "Links an Atom to the Atom representing the agent (a person, organization, bot, ...) that controls both."@en .


:interest rdfs:label "interest" ;
       rdfs:comment "Links the Atom representing an agent (a person, organization, bot, ...) to another Atom they control."@en .


:expertiseOf rdfs:label "expertiseOf" ;
        rdfs:comment "Links an Atom to the Atom representing the agent (a person, organization, bot, ...) that controls both."@en .


:expertise rdfs:label "expertise" ;
       rdfs:comment "Links the Atom representing an agent (a person, organization, bot, ...) to another Atom they control."@en .

#################################################################
#    General axioms
#################################################################

[ rdf:type owl:AllDifferent ;
  owl:distinctMembers ( :InterestOfSocket
                        :InterestSocket
                        :ExpertiseOfSocket
                        :ExpertiseSocket
                      )
] .
