@prefix : <https://w3id.org/won/auth#> .
@prefix owl: <http://www.w3.org/2002/07/owl#> .
@prefix rdf: <http://www.w3.org/1999/02/22-rdf-syntax-ns#> .
@prefix xml: <http://www.w3.org/XML/1998/namespace> .
@prefix xsd: <http://www.w3.org/2001/XMLSchema#> .
@prefix rdfs: <http://www.w3.org/2000/01/rdf-schema#> .
@base <https://w3id.org/won/auth#> .

<https://w3id.org/won/auth#> rdf:type owl:Ontology ;
                              owl:versionIRI <https://w3id.org/won/auth/1.0> ;
                              owl:imports <https://w3id.org/won/core> ,
                                          <https://w3id.org/won/msg> ;
                              <http://purl.org/dc/elements/1.1/abstract> "This vocabulary defines the terms used to express ACLs in WoN, as well as SHACL shapes for validating such ACLs."@en ;
                              <http://purl.org/dc/elements/1.1/creator> "Florian Kleedorfer" ;
                              <http://purl.org/dc/elements/1.1/title> "Web of Needs Authorization Vocabulary"@en ;
                              <http://purl.org/dc/terms/created> "2020-11-19"^^xsd:date ;
                              <http://purl.org/dc/terms/license> <https://creativecommons.org/licenses/by/4.0/> ;
                              <http://purl.org/vocab/vann/preferredNamespacePrefix> "auth" .

#################################################################
#    Annotation properties
#################################################################

###  http://www.w3.org/ns/shacl#class
<http://www.w3.org/ns/shacl#class> rdf:type owl:AnnotationProperty .


###  http://www.w3.org/ns/shacl#closed
<http://www.w3.org/ns/shacl#closed> rdf:type owl:AnnotationProperty .


###  http://www.w3.org/ns/shacl#datatype
<http://www.w3.org/ns/shacl#datatype> rdf:type owl:AnnotationProperty .


###  http://www.w3.org/ns/shacl#ignoredProperties
<http://www.w3.org/ns/shacl#ignoredProperties> rdf:type owl:AnnotationProperty .


###  http://www.w3.org/ns/shacl#in
<http://www.w3.org/ns/shacl#in> rdf:type owl:AnnotationProperty .


###  http://www.w3.org/ns/shacl#maxCount
<http://www.w3.org/ns/shacl#maxCount> rdf:type owl:AnnotationProperty .


###  http://www.w3.org/ns/shacl#minCount
<http://www.w3.org/ns/shacl#minCount> rdf:type owl:AnnotationProperty .


###  http://www.w3.org/ns/shacl#node
<http://www.w3.org/ns/shacl#node> rdf:type owl:AnnotationProperty .


###  http://www.w3.org/ns/shacl#nodeKind
<http://www.w3.org/ns/shacl#nodeKind> rdf:type owl:AnnotationProperty .


###  http://www.w3.org/ns/shacl#or
<http://www.w3.org/ns/shacl#or> rdf:type owl:AnnotationProperty .


###  http://www.w3.org/ns/shacl#path
<http://www.w3.org/ns/shacl#path> rdf:type owl:AnnotationProperty .


###  http://www.w3.org/ns/shacl#pattern
<http://www.w3.org/ns/shacl#pattern> rdf:type owl:AnnotationProperty .


###  http://www.w3.org/ns/shacl#property
<http://www.w3.org/ns/shacl#property> rdf:type owl:AnnotationProperty .


###  http://www.w3.org/ns/shacl#target
<http://www.w3.org/ns/shacl#target> rdf:type owl:AnnotationProperty .


###  http://www.w3.org/ns/shacl#targetClass
<http://www.w3.org/ns/shacl#targetClass> rdf:type owl:AnnotationProperty .


###  http://www.w3.org/ns/shacl#targetObjectsOf
<http://www.w3.org/ns/shacl#targetObjectsOf> rdf:type owl:AnnotationProperty .


###  http://www.w3.org/ns/shacl#targetSubjectsOf
<http://www.w3.org/ns/shacl#targetSubjectsOf> rdf:type owl:AnnotationProperty .


###  https://w3id.org/won/auth#AseLeafProperty
:AseLeafProperty rdf:type owl:AnnotationProperty ;
                 rdfs:domain :AtomStructureExpression .


###  https://w3id.org/won/auth#asePosition
:asePosition rdf:type owl:AnnotationProperty .


###  https://w3id.org/won/auth#inherit
:inherit rdf:type owl:AnnotationProperty ;
         rdfs:subPropertyOf :AseLeafProperty .


###  https://w3id.org/won/auth#label
:label rdf:type owl:AnnotationProperty .


###  https://w3id.org/won/auth#nodeSigned
:nodeSigned rdf:type owl:AnnotationProperty .


###  https://w3id.org/won/auth#operation
:operation rdf:type owl:AnnotationProperty ;
           rdfs:subPropertyOf :AseLeafProperty .


###  https://w3id.org/won/auth#parentPosition
:parentPosition rdf:type owl:AnnotationProperty .


###  https://w3id.org/won/auth#targetAtom
:targetAtom rdf:type owl:AnnotationProperty ;
            rdfs:subPropertyOf :AseLeafProperty .


#################################################################
#    Object Properties
#################################################################

###  https://w3id.org/won/auth#AseBranchProperty
:AseBranchProperty rdf:type owl:ObjectProperty ;
                   rdfs:domain :AtomStructureExpression ;
                   rdfs:range :AtomStructureExpression ;
                   rdfs:comment "Object properties of ASEs that have ASEs as their object."@en ;
                   rdfs:isDefinedBy <https://w3id.org/won/auth#> ;
                   rdfs:label "AseBranchProperty" .


###  https://w3id.org/won/auth#AseFilterProperty
:AseFilterProperty rdf:type owl:ObjectProperty ;
                   rdfs:domain :AtomStructureExpression .


###  https://w3id.org/won/auth#atom
:atom rdf:type owl:ObjectProperty ;
      rdfs:domain :AtomExpression ;
      rdfs:range [ rdf:type owl:Class ;
                   owl:unionOf rdf:nil
                 ] ;
      rdfs:comment "The relative or absolute reference to an atom."@en ;
      rdfs:isDefinedBy <https://w3id.org/won/auth#> ;
      rdfs:label "atom" .


###  https://w3id.org/won/auth#atomMessage
:atomMessage rdf:type owl:ObjectProperty ;
             rdfs:subPropertyOf :AseBranchProperty ;
             rdfs:domain [ rdf:type owl:Class ;
                           owl:unionOf rdf:nil
                         ] ;
             rdfs:range :AtomMessageExpression ;
             rdfs:comment """Used in the ASE root or atom messages expressions to specify a auth:AtomMessageExpression. The atom
     messages directly or transitively reachable from all target nodes become focus nodes of the atom message expression."""@en ;
             rdfs:isDefinedBy <https://w3id.org/won/auth#> ;
             rdfs:label "auth:atomMessage" .


###  https://w3id.org/won/auth#atomMessages
:atomMessages rdf:type owl:ObjectProperty ;
              rdfs:subPropertyOf :AseBranchProperty ;
              rdfs:domain :AseRoot ;
              rdfs:range :AtomMessagesExpression ;
              rdfs:comment """Used in the ASE root to specify a auth:AtomMessagesExpression. The atom message containers reachable from all target nodes 
    become focus nodes of the atom messages expression."""@en ;
              rdfs:isDefinedBy <https://w3id.org/won/auth#> ;
              rdfs:label "atomMessages" .


###  https://w3id.org/won/auth#atomState
:atomState rdf:type owl:ObjectProperty ;
           rdfs:subPropertyOf :AseFilterProperty ;
           rdfs:domain :AseRoot ;
           rdfs:range <https://w3id.org/won/core#AtomState> ;
           rdfs:comment "Filters focus nodes of the ASE root by atom state."@en ;
           rdfs:isDefinedBy <https://w3id.org/won/auth#> ;
           rdfs:label "atomState" .


###  https://w3id.org/won/auth#bearer
:bearer rdf:type owl:ObjectProperty ;
        rdfs:domain :Authorization ;
        rdfs:range :TokenShape ;
        rdfs:comment "Used in an Authorization to define constraints for tokens that if fulfilled, make their bearer a grantee."@en ;
        rdfs:isDefinedBy <https://w3id.org/won/auth#> ;
        rdfs:label "bearer" .


###  https://w3id.org/won/auth#connection
:connection rdf:type owl:ObjectProperty ;
            rdfs:subPropertyOf :AseBranchProperty ;
            rdfs:domain [ rdf:type owl:Class ;
                          owl:unionOf rdf:nil
                        ] ;
            rdfs:range :ConnectionExpression ;
            rdfs:comment "Used in the ASE root, socket or connections expressions to specify a auth:ConnectionExpression. The connections directly or transitively reachable from all target nodes become focus nodes of the connection expression."@en ;
            rdfs:isDefinedBy <https://w3id.org/won/auth#> ;
            rdfs:label "connection" .


###  https://w3id.org/won/auth#connectionIri
:connectionIri rdf:type owl:ObjectProperty ;
               rdfs:subPropertyOf :AseFilterProperty ;
               rdfs:domain :ConnectionExpression ;
               rdfs:range xsd:anyUri ;
               rdfs:comment "Filters focus nodes of the connection expression by connection IRI."@en ;
               rdfs:isDefinedBy <https://w3id.org/won/auth#> ;
               rdfs:label "connectionIri" .


###  https://w3id.org/won/auth#connectionMessage
:connectionMessage rdf:type owl:ObjectProperty ;
                   rdfs:subPropertyOf :AseBranchProperty ;
                   rdfs:domain [ rdf:type owl:Class ;
                                 owl:unionOf rdf:nil
                               ] ;
                   rdfs:range :ConnectionMessageExpression ;
                   rdfs:comment """Used in the ASE root, socket, connections, connection, or connection messages expressions to specify 
    a auth:ConnectionMessageExpression. The connection messages directly or transitively reachable from all target nodes 
    become focus nodes of the connection message expression."""@en ;
                   rdfs:isDefinedBy <https://w3id.org/won/auth#> ;
                   rdfs:label "connectionMessage" .


###  https://w3id.org/won/auth#connectionMessages
:connectionMessages rdf:type owl:ObjectProperty ;
                    rdfs:subPropertyOf :AseBranchProperty ;
                    rdfs:domain [ rdf:type owl:Class ;
                                  owl:unionOf rdf:nil
                                ] ;
                    rdfs:range :ConnectionMessagesExpression ;
                    rdfs:comment """Used in the ASE root, socket, connections, or connection expressions to specify 
    a auth:ConnectionMessagesExpression. The connection containers directly or transitively reachable from all target nodes 
    become focus nodes of the connection messages expression."""@en ;
                    rdfs:isDefinedBy <https://w3id.org/won/auth#> ;
                    rdfs:label "connectionMessages" .


###  https://w3id.org/won/auth#connectionState
:connectionState rdf:type owl:ObjectProperty ;
                 rdfs:subPropertyOf :AseFilterProperty ;
                 rdfs:domain [ rdf:type owl:Class ;
                               owl:unionOf rdf:nil
                             ] ;
                 rdfs:range <https://w3id.org/won/core#ConnectionState> ;
                 rdfs:comment "Filters focus nodes of the connection or connections expression by connection state."@en ;
                 rdfs:isDefinedBy <https://w3id.org/won/auth#> ;
                 rdfs:label "connectionState" .


###  https://w3id.org/won/auth#connections
:connections rdf:type owl:ObjectProperty ;
             rdfs:subPropertyOf :AseBranchProperty ;
             rdfs:domain [ rdf:type owl:Class ;
                           owl:unionOf rdf:nil
                         ] ;
             rdfs:range :ConnectionExpression ;
             rdfs:comment "Used in the ASE root or socket expressions to specify a auth:ConnectionsExpression. The connection containers directly or transitively reachable from all target nodes become focus nodes of the connections expression."@en ;
             rdfs:isDefinedBy <https://w3id.org/won/auth#> ;
             rdfs:label "connections" .


###  https://w3id.org/won/auth#decision
:decision rdf:type owl:ObjectProperty ;
          rdfs:domain :AclEvalResult ;
          rdfs:range :DecisionValue ;
          rdfs:comment "The decision (access granted or denied) made by evaluating the ACL."@en ;
          rdfs:isDefinedBy <https://w3id.org/won/auth#> ;
          rdfs:label "decision" .


###  https://w3id.org/won/auth#expiresAfter
:expiresAfter rdf:type owl:ObjectProperty ;
              rdfs:domain :TokenSpecification ;
              rdfs:range [ rdf:type owl:Class ;
                           owl:unionOf rdf:nil
                         ] .


###  https://w3id.org/won/auth#grant
:grant rdf:type owl:ObjectProperty ;
       rdfs:domain :Authorization ;
       rdfs:range :AseRoot ;
       rdfs:comment """An authorization defines the operations it grants in the form of an ASE tree annotated with
        auth:OperationExpressions using auth:grant."""@en ;
       rdfs:isDefinedBy <https://w3id.org/won/auth#> ;
       rdfs:label "grant" .


###  https://w3id.org/won/auth#grantee
:grantee rdf:type owl:ObjectProperty ;
         rdfs:domain :Authorization ;
         rdfs:range [ rdf:type owl:Class ;
                      owl:unionOf rdf:nil
                    ] ;
         rdfs:comment """Used in an Authorization to define the set of grantees. Linking to an ASE root means that the targets
        of auth:TargetAtomExpressions are grantees. Linking to an atom expression means that the targets of
        the atom expression are grantees. Linking to a granteeWildcard means any client is a grantee."""@en ;
         rdfs:isDefinedBy <https://w3id.org/won/auth#> ;
         rdfs:label "grantee" .


###  https://w3id.org/won/auth#graph
:graph rdf:type owl:ObjectProperty ;
       rdfs:domain :AseRoot ;
       rdfs:range :GraphExpression ;
       rdfs:comment "Used in the ASE root to specify a auth:GraphExpression."@en ;
       rdfs:isDefinedBy <https://w3id.org/won/auth#> ;
       rdfs:label "graph" .


###  https://w3id.org/won/auth#graphIri
:graphIri rdf:type owl:ObjectProperty ;
          rdfs:subPropertyOf :AseFilterProperty ;
          rdfs:domain :GraphExpression ;
          rdfs:comment "Filters focus nodes of the graph expression by graph IRI."@en ;
          rdfs:isDefinedBy <https://w3id.org/won/auth#> ;
          rdfs:label "graphIri" .


###  https://w3id.org/won/auth#graphType
:graphType rdf:type owl:ObjectProperty ;
           rdfs:subPropertyOf :AseFilterProperty ;
           rdfs:domain :GraphExpression ;
           rdfs:range :GraphType ;
           rdfs:comment "Filters focus nodes of the graph expression by graph type."@en ;
           rdfs:isDefinedBy <https://w3id.org/won/auth#> ;
           rdfs:label "graphType" .


###  https://w3id.org/won/auth#issueToken
:issueToken rdf:type owl:ObjectProperty ;
            rdfs:domain :AclEvalResult ;
            rdfs:range :AuthToken ;
            rdfs:comment "The token issued as the result of an ACL evaluation."@en ;
            rdfs:isDefinedBy <https://w3id.org/won/auth#> ;
            rdfs:label "issueToken" .


###  https://w3id.org/won/auth#issuer
:issuer rdf:type owl:ObjectProperty ;
        rdfs:domain [ rdf:type owl:Class ;
                      owl:unionOf rdf:nil
                    ] ;
        rdfs:range [ rdf:type owl:Class ;
                     owl:unionOf rdf:nil
                   ] ;
        rdfs:comment """auth:issuer is used to link indicate who did, was asked to, or is required as the issuer of a token.
    Note that it is not required that the issuer is identical with the signer of a token. Unless the property `auth:nodeSigned true` 
    is used, a token requested from an atom is signed by the WoN node on behalf of the atom. A token signed using
    the atom's private key can only be generated by the owner of the atom and thus involves a much more complex process
    to create."""@en ;
        rdfs:isDefinedBy <https://w3id.org/won/auth#> ;
        rdfs:label "issuer" .


###  https://w3id.org/won/auth#localAuth
:localAuth rdf:type owl:ObjectProperty ;
           rdfs:domain <https://w3id.org/won/core#SocketDefinition> ;
           rdfs:range :Authorization ;
           rdfs:comment "Authorization that a socket requests its own atom to add to its `#socket-acl` graph when it is added to the atom."@en ;
           rdfs:isDefinedBy <https://w3id.org/won/auth#> ;
           rdfs:label "localAuth" .


###  https://w3id.org/won/auth#messageOnBehalf
:messageOnBehalf rdf:type owl:ObjectProperty ;
                 rdfs:domain :MessageOperationExpression ;
                 rdfs:range [ rdf:type owl:Class ;
                              owl:unionOf rdf:nil
                            ] ;
                 rdfs:comment """Allows an auth:MessageOperationExpression to specify msg:MessageTypes that the grantee of the operation may
     send __on behalf__ of the actual atom owner, at the operation's position in the atom's tree structure. The message
     types are either listed as objects of auth:messageOnBealf or defined
     transitively. In the latter case, the object of auth:messageOnBehalf is an auth:MessageTypeSet, which in turn lists
     message types.
        """@en ;
                 rdfs:isDefinedBy <https://w3id.org/won/auth#> ;
                 rdfs:label "messageOnBehalf" .


###  https://w3id.org/won/auth#messageTo
:messageTo rdf:type owl:ObjectProperty ;
           rdfs:domain :MessageOperationExpression ;
           rdfs:range [ rdf:type owl:Class ;
                        owl:unionOf rdf:nil
                      ] ;
           rdfs:comment """Allows an auth:MessageOperationExpression to specify msg:MessageTypes that the grantee of the operation may
     send __to__ the atom, at the operation's position in the atom's tree structure. The message types are either
     listed as objects of auth:messageTo or defined transitively. In the latter case, the object of auth:messageTo
     is an auth:MessageTypeSet, which in turn lists message types.
        """@en ;
           rdfs:isDefinedBy <https://w3id.org/won/auth#> ;
           rdfs:label "messageTo" .


###  https://w3id.org/won/auth#operation
:operation rdf:type owl:ObjectProperty ;
           rdfs:range :OperationExpression .


###  https://w3id.org/won/auth#requestToken
:requestToken rdf:type owl:ObjectProperty ;
              rdfs:domain :TokenOperationExpression ;
              rdfs:range :TokenSpecification ;
              rdfs:comment "A TokenOperationExpression links to the specification of the requested token via auth:requestToken."@en ;
              rdfs:isDefinedBy <https://w3id.org/won/auth#> ;
              rdfs:label "requestToken" .


###  https://w3id.org/won/auth#requestedBy
:requestedBy rdf:type owl:ObjectProperty ;
             rdfs:domain :Authorization ;
             rdfs:range :Socket ;
             rdfs:comment """Sockets may define auth:Authorizaitons for the atoms they are added to and for the target atoms of
        connections that are made via the socket. These Authorizations are added to the atom's `#socket-acl` graph. In order
         to be able to remove the authorizations again when a socket is removed from the atom, the authorization links
         to the socket using auth:requestedBy."""@en ;
             rdfs:isDefinedBy <https://w3id.org/won/auth#> ;
             rdfs:label "requestedBy" .


###  https://w3id.org/won/auth#socket
:socket rdf:type owl:ObjectProperty ;
        rdfs:subPropertyOf :AseBranchProperty ;
        rdfs:domain :AseRoot ;
        rdfs:range :SocketExpression ;
        rdfs:comment "Used in the ASE root to specify a auth:SocketExpression. All sockets of the atom become focus nodes of the socket expression."@en ;
        rdfs:isDefinedBy <https://w3id.org/won/auth#> ;
        rdfs:label "socket" .


###  https://w3id.org/won/auth#socketIri
:socketIri rdf:type owl:ObjectProperty ;
           rdfs:subPropertyOf :AseFilterProperty ;
           rdfs:domain :SocketExpression ;
           rdfs:range xsd:anyUri ;
           rdfs:comment "Filters focus nodes of the socket expression by socket IRI (not to be confused with auth:socketType, which filters by IRI of the socket definition)."@en ;
           rdfs:isDefinedBy <https://w3id.org/won/auth#> ;
           rdfs:label "socketIri" .


###  https://w3id.org/won/auth#socketType
:socketType rdf:type owl:ObjectProperty ;
            rdfs:subPropertyOf :AseFilterProperty ;
            rdfs:domain :SocketExpression ;
            rdfs:range xsd:anyUri ;
            rdfs:comment "Filters focus nodes of the socket expression by socket definition IRI (not to be confused with auth:socketIri, which filters by IRI of the socket)."@en ;
            rdfs:isDefinedBy <https://w3id.org/won/auth#> ;
            rdfs:label "socketType" .


###  https://w3id.org/won/auth#targetAtom
:targetAtom rdf:type owl:ObjectProperty ;
            rdfs:domain :AtomStructureExpression .


###  https://w3id.org/won/auth#targetAuth
:targetAuth rdf:type owl:ObjectProperty ;
            rdfs:domain <https://w3id.org/won/core#SocketDefinition> ;
            rdfs:range :Authorization ;
            rdfs:comment "Authorization that a socket requests the target atoms of its connections to add to their `#socket-acl` graphs upon establishing a connection."@en ;
            rdfs:isDefinedBy <https://w3id.org/won/auth#> ;
            rdfs:label "targetAuth" .


###  https://w3id.org/won/auth#tokenExp
:tokenExp rdf:type owl:ObjectProperty ;
          rdfs:domain :AuthToken .


###  https://w3id.org/won/auth#tokenIat
:tokenIat rdf:type owl:ObjectProperty ;
          rdfs:domain :AuthToken .


###  https://w3id.org/won/auth#tokenIss
:tokenIss rdf:type owl:ObjectProperty ;
          rdfs:domain :AuthToken ;
          rdfs:range [ rdf:type owl:Class ;
                       owl:unionOf rdf:nil
                     ] ;
          rdfs:comment "The issuer of an actual token (either an atom uri or a won node uri)."@en ;
          rdfs:isDefinedBy <https://w3id.org/won/auth#> ;
          rdfs:label "tokenIss" .


###  https://w3id.org/won/auth#tokenScope
:tokenScope rdf:type owl:ObjectProperty ;
            rdfs:domain [ rdf:type owl:Class ;
                          owl:unionOf rdf:nil
                        ] ;
            rdfs:range [ rdf:type owl:Class ;
                         owl:unionOf rdf:nil
                       ] .


###  https://w3id.org/won/auth#tokenSub
:tokenSub rdf:type owl:ObjectProperty ;
          rdfs:domain :AuthToken ;
          rdfs:range [ rdf:type owl:Class ;
                       owl:unionOf rdf:nil
                     ] ;
          rdfs:comment "The subject of an actual token - the atom that requested it."@en ;
          rdfs:isDefinedBy <https://w3id.org/won/auth#> ;
          rdfs:label "tokenSub" .


#################################################################
#    Data properties
#################################################################

###  https://w3id.org/won/auth#expiresAfter
:expiresAfter rdf:type owl:DatatypeProperty .


###  https://w3id.org/won/auth#inherit
:inherit rdf:type owl:DatatypeProperty ;
         rdfs:range xsd:boolean .


###  https://w3id.org/won/auth#tokenExp
:tokenExp rdf:type owl:DatatypeProperty ;
          rdfs:range xsd:dateTime .


###  https://w3id.org/won/auth#tokenIat
:tokenIat rdf:type owl:DatatypeProperty ;
          rdfs:range xsd:dateTime .


###  https://w3id.org/won/auth#tokenScope
:tokenScope rdf:type owl:DatatypeProperty .


#################################################################
#    Classes
#################################################################

###  http://www.w3.org/2001/XMLSchema#anyUri
xsd:anyUri rdf:type owl:Class .


###  http://www.w3.org/ns/shacl#NodeShape
<http://www.w3.org/ns/shacl#NodeShape> rdf:type owl:Class .


###  http://www.w3.org/ns/shacl#PropertyShape
<http://www.w3.org/ns/shacl#PropertyShape> rdf:type owl:Class .


###  https://w3id.org/won/auth#AclEvalResult
:AclEvalResult rdf:type owl:Class ;
               rdfs:comment "Class of all authorization evaluation results, specifying a) the decision, b) granted auth tokens (if any), c) authInfo (if any)."@en ;
               rdfs:isDefinedBy <https://w3id.org/won/auth#> ;
               rdfs:label "AclEvalResult" .


###  https://w3id.org/won/auth#AseFilterProperty
:AseFilterProperty rdf:type owl:Class ;
                   rdfs:subClassOf :AseLeafProperty .


###  https://w3id.org/won/auth#AseLeafProperty
:AseLeafProperty rdf:type owl:Class .


###  https://w3id.org/won/auth#AsePosition
:AsePosition rdf:type owl:Class ;
             rdfs:comment "Class of all positions in the atom's tree structure"@en ;
             rdfs:isDefinedBy <https://w3id.org/won/auth#> ;
             rdfs:label "AsePosition" .


###  https://w3id.org/won/auth#AseRoot
:AseRoot rdf:type owl:Class ;
         rdfs:subClassOf :AtomStructureExpression ;
         rdfs:comment "Class of the roots of ASE trees"@en ;
         rdfs:isDefinedBy <https://w3id.org/won/auth#> ;
         rdfs:label "AseRoot" .


###  https://w3id.org/won/auth#AtomExpression
:AtomExpression rdf:type owl:Class ;
                rdfs:comment "An expression evaluating to an atom URI, either relative to some evaluation context or by its absolute URI."@en ;
                rdfs:isDefinedBy <https://w3id.org/won/auth#> ;
                rdfs:label "AtomExpression" .


###  https://w3id.org/won/auth#AtomMessageExpression
:AtomMessageExpression rdf:type owl:Class ;
                       rdfs:subClassOf :AtomStructureExpression ;
                       rdfs:comment "Class of all ASE that correspond to the atom message position in the atom tree structure."@en ;
                       rdfs:isDefinedBy <https://w3id.org/won/auth#> ;
                       rdfs:label "AtomMessageExpression" .


###  https://w3id.org/won/auth#AtomMessagesExpression
:AtomMessagesExpression rdf:type owl:Class ;
                        rdfs:subClassOf :AtomStructureExpression ;
                        rdfs:comment "Class of all ASE that correspond to the atom message container position in the atom tree structure."@en ;
                        rdfs:isDefinedBy <https://w3id.org/won/auth#> ;
                        rdfs:label "AtomMessagesExpression" .


###  https://w3id.org/won/auth#AtomStructureExpression
:AtomStructureExpression rdf:type owl:Class ;
                         rdfs:comment "Class of all atom structure expressions (ASEs)."@en ;
                         rdfs:isDefinedBy <https://w3id.org/won/auth#> ;
                         rdfs:label "AtomStructureExpression" .


###  https://w3id.org/won/auth#AuthToken
:AuthToken rdf:type owl:Class ;
           rdfs:comment "Class of all authentication tokens (when expressed in RDF, which makes sense for testing)."@en ;
           rdfs:isDefinedBy <https://w3id.org/won/auth#> ;
           rdfs:label "AuthToken" .


###  https://w3id.org/won/auth#Authorization
:Authorization rdf:type owl:Class ;
               rdfs:comment "Class of authorizations in WoN. Authorizations combine definitions of __who__ is allowed __what__ and if they are not, under which circumstances they may learn how to obtain access (i.e., get __authInfo__)."@en ;
               rdfs:isDefinedBy <https://w3id.org/won/auth#> ;
               rdfs:label "Authorization" .


###  https://w3id.org/won/auth#ConnectionExpression
:ConnectionExpression rdf:type owl:Class ;
                      rdfs:subClassOf :AtomStructureExpression ;
                      rdfs:comment "Class of all ASE that correspond to the connection position in the atom tree structure."@en ;
                      rdfs:isDefinedBy <https://w3id.org/won/auth#> ;
                      rdfs:label "ConnectionExpression" .


###  https://w3id.org/won/auth#ConnectionMessageExpression
:ConnectionMessageExpression rdf:type owl:Class ;
                             rdfs:subClassOf :AtomStructureExpression ;
                             rdfs:comment "Class of all ASE that correspond to the connection message position in the atom tree structure."@en ;
                             rdfs:isDefinedBy <https://w3id.org/won/auth#> ;
                             rdfs:label "ConnectionMessageExpression" .


###  https://w3id.org/won/auth#ConnectionMessagesExpression
:ConnectionMessagesExpression rdf:type owl:Class ;
                              rdfs:subClassOf :AtomStructureExpression ;
                              rdfs:comment "Class of all ASE that correspond to the connection message container position in the atom tree structure."@en ;
                              rdfs:isDefinedBy <https://w3id.org/won/auth#> ;
                              rdfs:label "ConnectionMessagesExpression" .


###  https://w3id.org/won/auth#ConnectionsExpression
:ConnectionsExpression rdf:type owl:Class ;
                       rdfs:subClassOf :AtomStructureExpression ;
                       rdfs:comment "Class of all ASE that correspond to the connection container position in the atom tree structure."@en ;
                       rdfs:isDefinedBy <https://w3id.org/won/auth#> ;
                       rdfs:label "ConnectionsExpression" .


###  https://w3id.org/won/auth#DecisionValue
:DecisionValue rdf:type owl:Class ;
               rdfs:comment "The class of autorization decisions (access denied or granted)"@en ;
               rdfs:isDefinedBy <https://w3id.org/won/auth#> ;
               rdfs:label "DecisionValue" .


###  https://w3id.org/won/auth#ExpectedAclEvalResult
:ExpectedAclEvalResult rdf:type owl:Class ;
                       rdfs:subClassOf :AclEvalResult ;
                       rdfs:comment "Class of expected authorization evaluation results, specifying a) the decision, b) granted auth tokens (if any), c) authInfo (if any)."@en ;
                       rdfs:isDefinedBy <https://w3id.org/won/auth#> ;
                       rdfs:label "ExpectedAclEvalResult" .


###  https://w3id.org/won/auth#GranteeWildcard
:GranteeWildcard rdf:type owl:Class ;
                 rdfs:comment "Expresses that any client is a grantee."@en ;
                 rdfs:isDefinedBy <https://w3id.org/won/auth#> ;
                 rdfs:label "GranteeWildcard" .


###  https://w3id.org/won/auth#GraphExpression
:GraphExpression rdf:type owl:Class ;
                 rdfs:subClassOf :AtomStructureExpression ;
                 rdfs:comment "Class of all ASE that correspond to the graph position in the atom tree structure."@en ;
                 rdfs:isDefinedBy <https://w3id.org/won/auth#> ;
                 rdfs:label "GraphExpression" .


###  https://w3id.org/won/auth#GraphType
:GraphType rdf:type owl:Class .


###  https://w3id.org/won/auth#InheritingShape
:InheritingShape rdf:type owl:Class ;
                 rdfs:comment "Class of all auth:TreeExpressionShape instances that inherit allowed operations from their parent and are thus allowed to use the auth:inherit property to block inheritance."@en ;
                 rdfs:isDefinedBy <https://w3id.org/won/auth#> ;
                 rdfs:label "InheritingShape" .


###  https://w3id.org/won/auth#MessageOperationExpression
:MessageOperationExpression rdf:type owl:Class ;
                            rdfs:subClassOf :OperationExpression ;
                            rdfs:comment "Class of all auth:OperationExpression instances that refer to sending messages."@en ;
                            rdfs:isDefinedBy <https://w3id.org/won/auth#> ;
                            rdfs:label "MessageOperationExpression" .


###  https://w3id.org/won/auth#MessageTypeSet
:MessageTypeSet rdf:type owl:Class ;
                rdfs:comment "Class of sets of msg:MessageType, identified by a resource, and listing message types via rdfs:member."@en ;
                rdfs:isDefinedBy <https://w3id.org/won/auth#> ;
                rdfs:label "MessageTypeSet" .


###  https://w3id.org/won/auth#MessageTypeSpecificationShape
:MessageTypeSpecificationShape rdf:type owl:Class .


###  https://w3id.org/won/auth#OperationContainerShape
:OperationContainerShape rdf:type owl:Class ;
                         rdfs:comment "Class of all auth:TreeExpressionShape instances thay may link to auth:OperationExpression instances via auth:operation."@en ;
                         rdfs:isDefinedBy <https://w3id.org/won/auth#> ;
                         rdfs:label "OperationContainerShape" .


###  https://w3id.org/won/auth#OperationExpression
:OperationExpression rdf:type owl:Class ;
                     rdfs:comment "Class of all WoN operations, such as reading the linked data representation of a resource, sending a message, etc."@en ;
                     rdfs:isDefinedBy <https://w3id.org/won/auth#> ;
                     rdfs:label "OperationExpression" .


###  https://w3id.org/won/auth#OperationExpressionShape
:OperationExpressionShape rdf:type owl:Class .


###  https://w3id.org/won/auth#RelativeAtomExpression
:RelativeAtomExpression rdf:type owl:Class ;
                        rdfs:subClassOf :AtomExpression ;
                        rdfs:comment "An expression evaluating to an atom URI relative to a given evaluation context."@en ;
                        rdfs:isDefinedBy <https://w3id.org/won/auth#> ;
                        rdfs:label "RelativeAtomExpression" .


###  https://w3id.org/won/auth#SimpleOperationExpression
:SimpleOperationExpression rdf:type owl:Class ;
                           rdfs:subClassOf :OperationExpression ;
                           rdfs:comment "Class of all auth:OperationExpression instances that require no further defining properties beyond their identifier."@en ;
                           rdfs:isDefinedBy <https://w3id.org/won/auth#> ;
                           rdfs:label "SimpleOperation" .


###  https://w3id.org/won/auth#Socket
:Socket rdf:type owl:Class .


###  https://w3id.org/won/auth#SocketExpression
:SocketExpression rdf:type owl:Class ;
                  rdfs:subClassOf :AtomStructureExpression ;
                  rdfs:comment "Class of all ASE that correspond to the socket position in the atom tree structure."@en ;
                  rdfs:isDefinedBy <https://w3id.org/won/auth#> ;
                  rdfs:label "SocketExpression" .


###  https://w3id.org/won/auth#TargetAtomContainerShape
:TargetAtomContainerShape rdf:type owl:Class ;
                          rdfs:comment "Class of all auth:TreeExpressionShape instances thay may contain a target atom expression via auth:targetAtom."@en ;
                          rdfs:isDefinedBy <https://w3id.org/won/auth#> ;
                          rdfs:label "TargetAtomContainerShape" .


###  https://w3id.org/won/auth#TokenOperationExpression
:TokenOperationExpression rdf:type owl:Class ;
                          rdfs:subClassOf :OperationExpression ;
                          rdfs:comment "Class of all auth:OperationExpression instances that refer to requesting an authentication token."@en ;
                          rdfs:isDefinedBy <https://w3id.org/won/auth#> ;
                          rdfs:label "TokenOperationExpression" .


###  https://w3id.org/won/auth#TokenScope
:TokenScope rdf:type owl:Class ;
            rdfs:comment "Class of all well-known token scopes. Using such scopes allows coordination across different domain ontologies." ;
            rdfs:isDefinedBy <https://w3id.org/won/auth#> ;
            rdfs:label "TokenScope" .


###  https://w3id.org/won/auth#TokenShape
:TokenShape rdf:type owl:Class ;
            rdfs:comment "Class of all definitions of token shapes, i.e. of specifications of the properties a token must have in order to be accepted."@en ;
            rdfs:isDefinedBy <https://w3id.org/won/auth#> ;
            rdfs:label "TokenShape" .


###  https://w3id.org/won/auth#TokenSpecification
:TokenSpecification rdf:type owl:Class ;
                    rdfs:comment "Class of all definition of tokens to be granted or tokens requested."@en ;
                    rdfs:isDefinedBy <https://w3id.org/won/auth#> ;
                    rdfs:label "TokenSpecification" .


###  https://w3id.org/won/auth#TreeExpressionShape
:TreeExpressionShape rdf:type owl:Class ;
                     rdfs:comment "Class of all SHACL shapes that specify atom structure expressions (ASEs)."@en ;
                     rdfs:isDefinedBy <https://w3id.org/won/auth#> ;
                     rdfs:label "TreeExpressionShape" .


#################################################################
#    Individuals
#################################################################

###  https://w3id.org/won/auth#OwnerToken
:OwnerToken rdf:type owl:NamedIndividual ,
                     :TokenScope ;
            rdfs:comment "URI reserved for the value of the scope claim of owner tokens" ;
            rdfs:isDefinedBy <https://w3id.org/won/auth#> .


###  https://w3id.org/won/auth#SocketDefinitionShape
:SocketDefinitionShape rdf:type owl:NamedIndividual ,
                                <http://www.w3.org/ns/shacl#NodeShape> ;
                       rdfs:isDefinedBy <https://w3id.org/won/auth#> ;
                       <http://www.w3.org/ns/shacl#property> :localAuthPropertyShape ,
                                                             :targetAuthPropertyShape ;
                       <http://www.w3.org/ns/shacl#targetClass> <https://w3id.org/won/core#SocketDefinition> .


###  https://w3id.org/won/auth#accessDenied
:accessDenied rdf:type owl:NamedIndividual ,
                       :DecisionValue ;
              rdfs:isDefinedBy <https://w3id.org/won/auth#> .


###  https://w3id.org/won/auth#accessGranted
:accessGranted rdf:type owl:NamedIndividual ,
                        :DecisionValue ;
               rdfs:isDefinedBy <https://w3id.org/won/auth#> .


###  https://w3id.org/won/auth#aclEvalResultShape
:aclEvalResultShape rdf:type owl:NamedIndividual ,
                             <http://www.w3.org/ns/shacl#NodeShape> ;
                    rdfs:isDefinedBy <https://w3id.org/won/auth#> ;
                    <http://www.w3.org/ns/shacl#class> :OperationResult ;
                    <http://www.w3.org/ns/shacl#property> _:genid18 ,
                                                          _:genid19 ,
                                                          _:genid20 ,
                                                          _:genid21 ,
                                                          _:genid22 ,
                                                          _:genid23 ;
                    <http://www.w3.org/ns/shacl#targetClass> :OperationResult .

_:genid18 <http://www.w3.org/ns/shacl#datatype> xsd:boolean ;
           <http://www.w3.org/ns/shacl#maxCount> 1 ;
           <http://www.w3.org/ns/shacl#nodeKind> <http://www.w3.org/ns/shacl#Literal> ;
           <http://www.w3.org/ns/shacl#path> :invalidToken .

_:genid19 <http://www.w3.org/ns/shacl#datatype> xsd:boolean ;
           <http://www.w3.org/ns/shacl#maxCount> 1 ;
           <http://www.w3.org/ns/shacl#nodeKind> <http://www.w3.org/ns/shacl#Literal> ;
           <http://www.w3.org/ns/shacl#path> :insufficientScope .

_:genid20 <http://www.w3.org/ns/shacl#maxCount> 1 ;
           <http://www.w3.org/ns/shacl#minCount> 1 ;
           <http://www.w3.org/ns/shacl#node> :operationRequestShape ;
           <http://www.w3.org/ns/shacl#nodeKind> <http://www.w3.org/ns/shacl#IRI> ;
           <http://www.w3.org/ns/shacl#path> :requestedOperation .

_:genid21 <http://www.w3.org/ns/shacl#maxCount> 1 ;
           <http://www.w3.org/ns/shacl#minCount> 1 ;
           <http://www.w3.org/ns/shacl#node> :decisionValueShape ;
           <http://www.w3.org/ns/shacl#nodeKind> <http://www.w3.org/ns/shacl#IRI> ;
           <http://www.w3.org/ns/shacl#path> :decision .

_:genid22 <http://www.w3.org/ns/shacl#maxCount> 1 ;
           <http://www.w3.org/ns/shacl#node> :authInfoShape ;
           <http://www.w3.org/ns/shacl#path> :provideAuthInfo .

_:genid23 <http://www.w3.org/ns/shacl#node> :authTokenShape ;
           <http://www.w3.org/ns/shacl#path> :issueToken .


###  https://w3id.org/won/auth#aclGraph
:aclGraph rdf:type owl:NamedIndividual ,
                   :GraphType ;
          rdfs:isDefinedBy <https://w3id.org/won/auth#> .


###  https://w3id.org/won/auth#anyAtom
:anyAtom rdf:type owl:NamedIndividual ,
                  :RelativeAtomExpression ;
         rdfs:isDefinedBy <https://w3id.org/won/auth#> .


###  https://w3id.org/won/auth#anyMessageType
:anyMessageType rdf:type owl:NamedIndividual ;
                rdfs:isDefinedBy <https://w3id.org/won/auth#> .


###  https://w3id.org/won/auth#anyOperation
:anyOperation rdf:type owl:NamedIndividual ,
                       :SimpleOperationExpression ;
              rdfs:isDefinedBy <https://w3id.org/won/auth#> .


###  https://w3id.org/won/auth#anyone
:anyone rdf:type owl:NamedIndividual ,
                 :GranteeWildcard ;
        rdfs:isDefinedBy <https://w3id.org/won/auth#> .


###  https://w3id.org/won/auth#asePositionShape
:asePositionShape rdf:type owl:NamedIndividual ,
                           <http://www.w3.org/ns/shacl#NodeShape> ;
                  rdfs:isDefinedBy <https://w3id.org/won/auth#> ;
                  <http://www.w3.org/ns/shacl#ignoredProperties> [ ] ;
<http://www.w3.org/ns/shacl#in> [ ] ;
<http://www.w3.org/ns/shacl#property> _:genid26 ;
<http://www.w3.org/ns/shacl#targetClass> :AsePosition .

_:genid26 <http://www.w3.org/ns/shacl#class> :AsePosition ;
           <http://www.w3.org/ns/shacl#maxCount> 1 ;
           <http://www.w3.org/ns/shacl#path> :parentPosition .


###  https://w3id.org/won/auth#aseRootShape
:aseRootShape rdf:type owl:NamedIndividual ,
                       <http://www.w3.org/ns/shacl#NodeShape> ,
                       :OperationContainerShape ,
                       :TargetAtomContainerShape ,
                       :TreeExpressionShape ;
              rdfs:isDefinedBy <https://w3id.org/won/auth#> ;
              <http://www.w3.org/ns/shacl#closed> "true"^^xsd:boolean ;
              <http://www.w3.org/ns/shacl#ignoredProperties> [ ] ;
<http://www.w3.org/ns/shacl#nodeKind> <http://www.w3.org/ns/shacl#BlankNodeOrIRI> ;
<http://www.w3.org/ns/shacl#or> [ ] ;
:asePosition :positionRoot .


###  https://w3id.org/won/auth#atomExpressionShape
:atomExpressionShape rdf:type owl:NamedIndividual ,
                              <http://www.w3.org/ns/shacl#NodeShape> ;
                     rdfs:isDefinedBy <https://w3id.org/won/auth#> ;
                     <http://www.w3.org/ns/shacl#closed> "true"^^xsd:boolean ;
                     <http://www.w3.org/ns/shacl#ignoredProperties> [ ] ;
<http://www.w3.org/ns/shacl#property> _:genid30 ;
<http://www.w3.org/ns/shacl#targetSubjectsOf> :atom .

_:genid30 <http://www.w3.org/ns/shacl#minCount> 1 ;
           <http://www.w3.org/ns/shacl#or> [ ] ;
<http://www.w3.org/ns/shacl#path> :atom .


###  https://w3id.org/won/auth#atomMessageExpressionShape
:atomMessageExpressionShape rdf:type owl:NamedIndividual ,
                                     <http://www.w3.org/ns/shacl#NodeShape> ,
                                     :InheritingShape ,
                                     :OperationContainerShape ,
                                     :TreeExpressionShape ;
                            rdfs:isDefinedBy <https://w3id.org/won/auth#> ;
                            <http://www.w3.org/ns/shacl#closed> "true"^^xsd:boolean ;
                            <http://www.w3.org/ns/shacl#ignoredProperties> [ ] ;
<http://www.w3.org/ns/shacl#or> [ ] ;
:asePosition :positionAtomMessage .


###  https://w3id.org/won/auth#atomMessagePropertyShape
:atomMessagePropertyShape rdf:type owl:NamedIndividual ,
                                   <http://www.w3.org/ns/shacl#PropertyShape> ;
                          rdfs:isDefinedBy <https://w3id.org/won/auth#> ;
                          <http://www.w3.org/ns/shacl#minCount> 1 ;
                          <http://www.w3.org/ns/shacl#node> :atomMessageExpressionShape ;
                          <http://www.w3.org/ns/shacl#path> :atomMessage .


###  https://w3id.org/won/auth#atomMessagesExpressionShape
:atomMessagesExpressionShape rdf:type owl:NamedIndividual ,
                                      <http://www.w3.org/ns/shacl#NodeShape> ,
                                      :InheritingShape ,
                                      :OperationContainerShape ,
                                      :TreeExpressionShape ;
                             rdfs:isDefinedBy <https://w3id.org/won/auth#> ;
                             <http://www.w3.org/ns/shacl#closed> "true"^^xsd:boolean ;
                             <http://www.w3.org/ns/shacl#ignoredProperties> [ ] ;
<http://www.w3.org/ns/shacl#or> [ ] ;
:asePosition :positionAtomMessages .


###  https://w3id.org/won/auth#atomMessagesPropertyShape
:atomMessagesPropertyShape rdf:type owl:NamedIndividual ,
                                    <http://www.w3.org/ns/shacl#PropertyShape> ;
                           rdfs:isDefinedBy <https://w3id.org/won/auth#> ;
                           <http://www.w3.org/ns/shacl#minCount> 1 ;
                           <http://www.w3.org/ns/shacl#node> :atomMessagesExpressionShape ;
                           <http://www.w3.org/ns/shacl#path> :atomMessages .


###  https://w3id.org/won/auth#atomStatePropertyShape
:atomStatePropertyShape rdf:type owl:NamedIndividual ,
                                 <http://www.w3.org/ns/shacl#PropertyShape> ;
                        rdfs:isDefinedBy <https://w3id.org/won/auth#> ;
                        <http://www.w3.org/ns/shacl#minCount> 1 ;
                        <http://www.w3.org/ns/shacl#node> :atomStateShape ;
                        <http://www.w3.org/ns/shacl#path> :atomState .


###  https://w3id.org/won/auth#atomStateShape
:atomStateShape rdf:type owl:NamedIndividual ,
                         <http://www.w3.org/ns/shacl#NodeShape> ;
                rdfs:isDefinedBy <https://w3id.org/won/auth#> ;
                <http://www.w3.org/ns/shacl#closed> "true"^^xsd:boolean ;
                <http://www.w3.org/ns/shacl#in> [ ] ;
<http://www.w3.org/ns/shacl#nodeKind> <http://www.w3.org/ns/shacl#IRI> .


###  https://w3id.org/won/auth#authInfoShape
:authInfoShape rdf:type owl:NamedIndividual ,
                        <http://www.w3.org/ns/shacl#NodeShape> ;
               rdfs:isDefinedBy <https://w3id.org/won/auth#> ;
               <http://www.w3.org/ns/shacl#closed> "true"^^xsd:boolean ;
               <http://www.w3.org/ns/shacl#ignoredProperties> [ ] ;
<http://www.w3.org/ns/shacl#or> [ ] ;
<http://www.w3.org/ns/shacl#targetClass> :AuthInfo .


###  https://w3id.org/won/auth#authTokenShape
:authTokenShape rdf:type owl:NamedIndividual ,
                         <http://www.w3.org/ns/shacl#NodeShape> ;
                rdfs:isDefinedBy <https://w3id.org/won/auth#> ;
                <http://www.w3.org/ns/shacl#property> :tokenExpPropertyShape ,
                                                      :tokenIatPropertyShape ,
                                                      :tokenIssPropertyShape ,
                                                      :tokenScopePropertyShape ,
                                                      :tokenSigPropertyShape ,
                                                      :tokenSubPropertyShape ;
                <http://www.w3.org/ns/shacl#targetClass> :AuthToken .


###  https://w3id.org/won/auth#authTokenTestSpecShape
:authTokenTestSpecShape rdf:type owl:NamedIndividual ,
                                 <http://www.w3.org/ns/shacl#NodeShape> ;
                        rdfs:isDefinedBy <https://w3id.org/won/auth#> ;
                        <http://www.w3.org/ns/shacl#property> :expiresAfterPropertyShape ,
                                                              :tokenIssPropertyShape ,
                                                              :tokenScopePropertyShape ,
                                                              :tokenSigPropertyShape ,
                                                              :tokenSubPropertyShape .


###  https://w3id.org/won/auth#authorizationRequestor
:authorizationRequestor rdf:type owl:NamedIndividual ,
                                 :RelativeAtomExpression ;
                        rdfs:isDefinedBy <https://w3id.org/won/auth#> .


###  https://w3id.org/won/auth#authorizationShape
:authorizationShape rdf:type owl:NamedIndividual ,
                             <http://www.w3.org/ns/shacl#NodeShape> ;
                    rdfs:isDefinedBy <https://w3id.org/won/auth#> ;
                    <http://www.w3.org/ns/shacl#class> :Authorization ;
                    <http://www.w3.org/ns/shacl#closed> "true"^^xsd:boolean ;
                    <http://www.w3.org/ns/shacl#ignoredProperties> [ ] ;
<http://www.w3.org/ns/shacl#or> [ ] ,
[ ] ;
<http://www.w3.org/ns/shacl#property> _:genid42 ;
<http://www.w3.org/ns/shacl#targetClass> :Authorization .

_:genid42 <http://www.w3.org/ns/shacl#nodeKind> <http://www.w3.org/ns/shacl#IRI> ;
           <http://www.w3.org/ns/shacl#path> :requestedBy .


###  https://w3id.org/won/auth#connectionExpressionShape
:connectionExpressionShape rdf:type owl:NamedIndividual ,
                                    <http://www.w3.org/ns/shacl#NodeShape> ,
                                    :InheritingShape ,
                                    :OperationContainerShape ,
                                    :TargetAtomContainerShape ,
                                    :TreeExpressionShape ;
                           rdfs:isDefinedBy <https://w3id.org/won/auth#> ;
                           <http://www.w3.org/ns/shacl#closed> "true"^^xsd:boolean ;
                           <http://www.w3.org/ns/shacl#ignoredProperties> [ ] ;
<http://www.w3.org/ns/shacl#or> [ ] ;
<http://www.w3.org/ns/shacl#targetObjectsOf> :connection ;
:asePosition :positionConnection .


###  https://w3id.org/won/auth#connectionMessageExpressionShape
:connectionMessageExpressionShape rdf:type owl:NamedIndividual ,
                                           <http://www.w3.org/ns/shacl#NodeShape> ,
                                           :InheritingShape ,
                                           :OperationContainerShape ,
                                           :TreeExpressionShape ;
                                  rdfs:isDefinedBy <https://w3id.org/won/auth#> ;
                                  <http://www.w3.org/ns/shacl#closed> "true"^^xsd:boolean ;
                                  <http://www.w3.org/ns/shacl#ignoredProperties> [ ] ;
<http://www.w3.org/ns/shacl#or> [ ] ;
:asePosition :positionConnectionMessage .


###  https://w3id.org/won/auth#connectionMessagePropertyShape
:connectionMessagePropertyShape rdf:type owl:NamedIndividual ,
                                         <http://www.w3.org/ns/shacl#PropertyShape> ;
                                rdfs:isDefinedBy <https://w3id.org/won/auth#> ;
                                <http://www.w3.org/ns/shacl#minCount> 1 ;
                                <http://www.w3.org/ns/shacl#node> :connectionMessageExpressionShape ;
                                <http://www.w3.org/ns/shacl#path> :connectionMessage .


###  https://w3id.org/won/auth#connectionMessagesExpressionShape
:connectionMessagesExpressionShape rdf:type owl:NamedIndividual ,
                                            <http://www.w3.org/ns/shacl#NodeShape> ,
                                            :InheritingShape ,
                                            :OperationContainerShape ,
                                            :TreeExpressionShape ;
                                   rdfs:isDefinedBy <https://w3id.org/won/auth#> ;
                                   <http://www.w3.org/ns/shacl#closed> "true"^^xsd:boolean ;
                                   <http://www.w3.org/ns/shacl#ignoredProperties> [ ] ;
<http://www.w3.org/ns/shacl#or> [ ] ;
:asePosition :positionConnectionMessages .


###  https://w3id.org/won/auth#connectionMessagesPropertyShape
:connectionMessagesPropertyShape rdf:type owl:NamedIndividual ,
                                          <http://www.w3.org/ns/shacl#PropertyShape> ;
                                 rdfs:isDefinedBy <https://w3id.org/won/auth#> ;
                                 <http://www.w3.org/ns/shacl#minCount> 1 ;
                                 <http://www.w3.org/ns/shacl#node> :connectionMessagesExpressionShape ;
                                 <http://www.w3.org/ns/shacl#path> :connectionMessages .


###  https://w3id.org/won/auth#connectionPropertyShape
:connectionPropertyShape rdf:type owl:NamedIndividual ,
                                  <http://www.w3.org/ns/shacl#PropertyShape> ;
                         rdfs:isDefinedBy <https://w3id.org/won/auth#> ;
                         <http://www.w3.org/ns/shacl#minCount> 1 ;
                         <http://www.w3.org/ns/shacl#node> :connectionExpressionShape ;
                         <http://www.w3.org/ns/shacl#path> :connection .


###  https://w3id.org/won/auth#connectionStateShape
:connectionStateShape rdf:type owl:NamedIndividual ,
                               <http://www.w3.org/ns/shacl#NodeShape> ;
                      rdfs:isDefinedBy <https://w3id.org/won/auth#> ;
                      <http://www.w3.org/ns/shacl#closed> "true"^^xsd:boolean ;
                      <http://www.w3.org/ns/shacl#in> [ ] .


###  https://w3id.org/won/auth#connectionsExpressionShape
:connectionsExpressionShape rdf:type owl:NamedIndividual ,
                                     <http://www.w3.org/ns/shacl#NodeShape> ,
                                     :InheritingShape ,
                                     :OperationContainerShape ,
                                     :TargetAtomContainerShape ,
                                     :TreeExpressionShape ;
                            rdfs:isDefinedBy <https://w3id.org/won/auth#> ;
                            <http://www.w3.org/ns/shacl#closed> "true"^^xsd:boolean ;
                            <http://www.w3.org/ns/shacl#ignoredProperties> [ ] ;
<http://www.w3.org/ns/shacl#or> [ ] ;
<http://www.w3.org/ns/shacl#targetObjectsOf> :connections ;
:asePosition :positionConnections .


###  https://w3id.org/won/auth#connectionsPropertyShape
:connectionsPropertyShape rdf:type owl:NamedIndividual ,
                                   <http://www.w3.org/ns/shacl#PropertyShape> ;
                          rdfs:isDefinedBy <https://w3id.org/won/auth#> ;
                          <http://www.w3.org/ns/shacl#minCount> 1 ;
                          <http://www.w3.org/ns/shacl#node> :connectionsExpressionShape ;
                          <http://www.w3.org/ns/shacl#path> :connections .


###  https://w3id.org/won/auth#contentGraph
:contentGraph rdf:type owl:NamedIndividual ,
                       :GraphType ;
              rdfs:isDefinedBy <https://w3id.org/won/auth#> .


###  https://w3id.org/won/auth#decisionValueShape
:decisionValueShape rdf:type owl:NamedIndividual ,
                             <http://www.w3.org/ns/shacl#NodeShape> ;
                    rdfs:isDefinedBy <https://w3id.org/won/auth#> ;
                    <http://www.w3.org/ns/shacl#closed> "true"^^xsd:boolean ;
                    <http://www.w3.org/ns/shacl#ignoredProperties> [ ] ;
<http://www.w3.org/ns/shacl#in> [ ] .


###  https://w3id.org/won/auth#ensureShapesGraphIsAddedToDataGraph1
:ensureShapesGraphIsAddedToDataGraph1 rdf:type owl:NamedIndividual ,
                                               <http://www.w3.org/ns/shacl#NodeShape> ;
                                      rdfs:isDefinedBy <https://w3id.org/won/auth#> ;
                                      <http://www.w3.org/ns/shacl#class> :SimpleOperationExpression ;
                                      <http://www.w3.org/ns/shacl#target> :anyOperation ,
                                                                          :opRead .


###  https://w3id.org/won/auth#expectedAclEvalResultShape
:expectedAclEvalResultShape rdf:type owl:NamedIndividual ,
                                     <http://www.w3.org/ns/shacl#NodeShape> ;
                            rdfs:isDefinedBy <https://w3id.org/won/auth#> ;
                            <http://www.w3.org/ns/shacl#class> :ExpectedAclEvalResult ;
                            <http://www.w3.org/ns/shacl#property> _:genid54 ,
                                                                  _:genid55 ,
                                                                  _:genid56 ,
                                                                  _:genid57 ;
                            <http://www.w3.org/ns/shacl#targetClass> :ExpectedAclEvalResult .

_:genid54 <http://www.w3.org/ns/shacl#maxCount> 1 ;
           <http://www.w3.org/ns/shacl#minCount> 1 ;
           <http://www.w3.org/ns/shacl#node> :operationRequestShape ;
           <http://www.w3.org/ns/shacl#nodeKind> <http://www.w3.org/ns/shacl#IRI> ;
           <http://www.w3.org/ns/shacl#path> :requestedOperation .

_:genid55 <http://www.w3.org/ns/shacl#maxCount> 1 ;
           <http://www.w3.org/ns/shacl#minCount> 1 ;
           <http://www.w3.org/ns/shacl#node> :decisionValueShape ;
           <http://www.w3.org/ns/shacl#nodeKind> <http://www.w3.org/ns/shacl#IRI> ;
           <http://www.w3.org/ns/shacl#path> :decision .

_:genid56 <http://www.w3.org/ns/shacl#node> :authTokenTestSpecShape ;
           <http://www.w3.org/ns/shacl#path> :issueToken .

_:genid57 <http://www.w3.org/ns/shacl#maxCount> 1 ;
           <http://www.w3.org/ns/shacl#node> :authInfoShape ;
           <http://www.w3.org/ns/shacl#path> :provideAuthInfo .


###  https://w3id.org/won/auth#expiresAfterPropertyShape
:expiresAfterPropertyShape rdf:type owl:NamedIndividual ,
                                    <http://www.w3.org/ns/shacl#PropertyShape> ;
                           rdfs:isDefinedBy <https://w3id.org/won/auth#> ;
                           <http://www.w3.org/ns/shacl#maxCount> 1 ;
                           <http://www.w3.org/ns/shacl#nodeKind> <http://www.w3.org/ns/shacl#Literal> ;
                           <http://www.w3.org/ns/shacl#or> [ ] ;
<http://www.w3.org/ns/shacl#path> :expiresAfter .


###  https://w3id.org/won/auth#grantOwnerTokenToOwner
:grantOwnerTokenToOwner rdf:type owl:NamedIndividual ,
                                 :Authorization ;
                        :grant _:genid59 ;
                        :grantee _:genid62 ;
                        rdfs:isDefinedBy <https://w3id.org/won/auth#> .

_:genid59 :operation _:genid60 .

_:genid62 :atom :self .

_:genid60 :requestToken _:genid61 .

_:genid61 :tokenScope :OwnerToken ;
           :expiresAfter 3600 ;
           :nodeSigned "true"^^xsd:boolean .


###  https://w3id.org/won/auth#granteeWildcardShape
:granteeWildcardShape rdf:type owl:NamedIndividual ,
                               <http://www.w3.org/ns/shacl#NodeShape> ;
                      rdfs:isDefinedBy <https://w3id.org/won/auth#> ;
                      <http://www.w3.org/ns/shacl#closed> "true"^^xsd:boolean ;
                      <http://www.w3.org/ns/shacl#ignoredProperties> [ ] ;
<http://www.w3.org/ns/shacl#in> [ ] ;
<http://www.w3.org/ns/shacl#nodeKind> <http://www.w3.org/ns/shacl#IRI> .


###  https://w3id.org/won/auth#grantsForConnStateClosed
:grantsForConnStateClosed rdf:type owl:NamedIndividual ,
                                   :Authorization ;
                          :grant _:genid65 ;
                          :grantee _:genid68 ;
                          rdfs:isDefinedBy <https://w3id.org/won/auth#> .

_:genid65 :connection _:genid66 .

_:genid68 :connection _:genid69 .

_:genid66 :operation :opConnectClose ;
           :targetAtom _:genid67 .

_:genid69 :connectionState <https://w3id.org/won/core#Closed> ;
           :targetAtom [ ] .

_:genid67 :atom :operationRequestor .


###  https://w3id.org/won/auth#grantsForConnStateConnected
:grantsForConnStateConnected rdf:type owl:NamedIndividual ,
                                      :Authorization ;
                             :grant _:genid71 ;
                             :grantee _:genid75 ;
                             rdfs:isDefinedBy <https://w3id.org/won/auth#> .

_:genid71 :connection _:genid72 ;
           :graph _:genid74 .

_:genid75 :connection _:genid76 .

_:genid72 :operation :opCommunicate ;
           :targetAtom _:genid73 .

_:genid74 :graphType :contentGraph ,
                      :keyGraph ,
                      :sysinfoGraph ;
           :operation :opRead .

_:genid76 :connectionState <https://w3id.org/won/core#Connected> ;
           :targetAtom [ ] .

_:genid73 :atom :operationRequestor .


###  https://w3id.org/won/auth#grantsForConnStateRequestReceived
:grantsForConnStateRequestReceived rdf:type owl:NamedIndividual ,
                                            :Authorization ;
                                   :grant _:genid78 ;
                                   :grantee _:genid82 ;
                                   rdfs:isDefinedBy <https://w3id.org/won/auth#> .

_:genid78 :connection _:genid79 ;
           :graph _:genid81 .

_:genid82 :connection _:genid83 .

_:genid79 :operation :opConnectClose ;
           :targetAtom _:genid80 .

_:genid81 :graphType :contentGraph ,
                      :keyGraph ,
                      :sysinfoGraph ;
           :operation :opRead .

_:genid83 :connectionState <https://w3id.org/won/core#RequestReceived> ;
           :targetAtom [ ] .

_:genid80 :atom :operationRequestor .


###  https://w3id.org/won/auth#grantsForConnStateRequestSent
:grantsForConnStateRequestSent rdf:type owl:NamedIndividual ,
                                        :Authorization ;
                               :grant _:genid85 ;
                               :grantee _:genid89 ;
                               rdfs:isDefinedBy <https://w3id.org/won/auth#> .

_:genid85 :connection _:genid86 ;
           :graph _:genid88 .

_:genid89 :connection _:genid90 .

_:genid86 :operation :opConnectClose ;
           :targetAtom _:genid87 .

_:genid88 :graphType :contentGraph ,
                      :keyGraph ,
                      :sysinfoGraph ;
           :operation :opRead .

_:genid90 :connectionState <https://w3id.org/won/core#RequestSent> ;
           :targetAtom [ ] .

_:genid87 :atom :operationRequestor .


###  https://w3id.org/won/auth#grantsForOwnerTokenBearer
:grantsForOwnerTokenBearer rdf:type owl:NamedIndividual ,
                                    :Authorization ;
                           :bearer _:genid92 ;
                           :grant _:genid94 ;
                           rdfs:isDefinedBy <https://w3id.org/won/auth#> .

_:genid92 :issuer _:genid93 ;
           :tokenScope :OwnerToken ;
           :nodeSigned "true"^^xsd:boolean .

_:genid94 :operation :anyOperation .

_:genid93 :atom :self .


###  https://w3id.org/won/auth#graphExpressionShape
:graphExpressionShape rdf:type owl:NamedIndividual ,
                               <http://www.w3.org/ns/shacl#NodeShape> ,
                               :InheritingShape ,
                               :OperationContainerShape ,
                               :TreeExpressionShape ;
                      rdfs:isDefinedBy <https://w3id.org/won/auth#> ;
                      <http://www.w3.org/ns/shacl#closed> "true"^^xsd:boolean ;
                      <http://www.w3.org/ns/shacl#ignoredProperties> [ ] ;
<http://www.w3.org/ns/shacl#or> [ ] ;
:asePosition :positionAtomGraph .


###  https://w3id.org/won/auth#graphPropertyShape
:graphPropertyShape rdf:type owl:NamedIndividual ,
                             <http://www.w3.org/ns/shacl#PropertyShape> ;
                    rdfs:isDefinedBy <https://w3id.org/won/auth#> ;
                    <http://www.w3.org/ns/shacl#minCount> 1 ;
                    <http://www.w3.org/ns/shacl#node> :graphExpressionShape ;
                    <http://www.w3.org/ns/shacl#path> :graph .


###  https://w3id.org/won/auth#graphTypeShape
:graphTypeShape rdf:type owl:NamedIndividual ,
                         <http://www.w3.org/ns/shacl#NodeShape> ;
                rdfs:isDefinedBy <https://w3id.org/won/auth#> ;
                <http://www.w3.org/ns/shacl#closed> "true"^^xsd:boolean ;
                <http://www.w3.org/ns/shacl#ignoredProperties> [ ] ;
<http://www.w3.org/ns/shacl#in> [ ] .


###  https://w3id.org/won/auth#inheritPropertyShape
:inheritPropertyShape rdf:type owl:NamedIndividual ,
                               <http://www.w3.org/ns/shacl#PropertyShape> ;
                      rdfs:isDefinedBy <https://w3id.org/won/auth#> ;
                      <http://www.w3.org/ns/shacl#datatype> xsd:boolean ;
                      <http://www.w3.org/ns/shacl#maxCount> 1 ;
                      <http://www.w3.org/ns/shacl#path> :inherit .


###  https://w3id.org/won/auth#keyGraph
:keyGraph rdf:type owl:NamedIndividual ,
                   :GraphType ;
          rdfs:isDefinedBy <https://w3id.org/won/auth#> .


###  https://w3id.org/won/auth#localAuthPropertyShape
:localAuthPropertyShape rdf:type owl:NamedIndividual ,
                                 <http://www.w3.org/ns/shacl#PropertyShape> ;
                        rdfs:isDefinedBy <https://w3id.org/won/auth#> ;
                        <http://www.w3.org/ns/shacl#node> :authorizationShape ;
                        <http://www.w3.org/ns/shacl#path> :localAuth .


###  https://w3id.org/won/auth#messageOperationExpressionShape
:messageOperationExpressionShape rdf:type owl:NamedIndividual ,
                                          <http://www.w3.org/ns/shacl#NodeShape> ,
                                          :OperationExpressionShape ;
                                 rdfs:isDefinedBy <https://w3id.org/won/auth#> ;
                                 <http://www.w3.org/ns/shacl#closed> "true"^^xsd:boolean ;
                                 <http://www.w3.org/ns/shacl#ignoredProperties> [ ] ;
<http://www.w3.org/ns/shacl#or> [ ] ;
<http://www.w3.org/ns/shacl#targetClass> :MessageOperationExpression .


###  https://w3id.org/won/auth#messageTypeShape
:messageTypeShape rdf:type owl:NamedIndividual ,
                           <http://www.w3.org/ns/shacl#NodeShape> ,
                           :MessageTypeSpecificationShape ;
                  rdfs:isDefinedBy <https://w3id.org/won/auth#> ;
                  <http://www.w3.org/ns/shacl#closed> "true"^^xsd:boolean ;
                  <http://www.w3.org/ns/shacl#in> [ ] .


###  https://w3id.org/won/auth#messageTypesExpressionShape
:messageTypesExpressionShape rdf:type owl:NamedIndividual ,
                                      <http://www.w3.org/ns/shacl#NodeShape> ,
                                      :MessageTypeSpecificationShape ;
                             rdfs:isDefinedBy <https://w3id.org/won/auth#> ;
                             <http://www.w3.org/ns/shacl#property> _:genid102 ;
                             <http://www.w3.org/ns/shacl#targetClass> :MessageTypeSet .

_:genid102 <http://www.w3.org/ns/shacl#minCount> 1 ;
            <http://www.w3.org/ns/shacl#node> :messageTypeShape ;
            <http://www.w3.org/ns/shacl#path> rdfs:member .


###  https://w3id.org/won/auth#messageWildcardShape
:messageWildcardShape rdf:type owl:NamedIndividual ,
                               <http://www.w3.org/ns/shacl#NodeShape> ,
                               :MessageTypeSpecificationShape ;
                      rdfs:isDefinedBy <https://w3id.org/won/auth#> ;
                      <http://www.w3.org/ns/shacl#closed> "true"^^xsd:boolean ;
                      <http://www.w3.org/ns/shacl#ignoredProperties> [ ] ;
<http://www.w3.org/ns/shacl#in> [ ] ;
<http://www.w3.org/ns/shacl#nodeKind> <http://www.w3.org/ns/shacl#IRI> .


###  https://w3id.org/won/auth#msgTypesCommunicate
:msgTypesCommunicate rdf:type owl:NamedIndividual ,
                              :MessageTypeSet ;
                     rdfs:isDefinedBy <https://w3id.org/won/auth#> .


###  https://w3id.org/won/auth#msgTypesConnectClose
:msgTypesConnectClose rdf:type owl:NamedIndividual ,
                               :MessageTypeSet ;
                      rdfs:isDefinedBy <https://w3id.org/won/auth#> .


###  https://w3id.org/won/auth#msgTypesHint
:msgTypesHint rdf:type owl:NamedIndividual ,
                       :MessageTypeSet ;
              rdfs:isDefinedBy <https://w3id.org/won/auth#> .


###  https://w3id.org/won/auth#msgTypesModify
:msgTypesModify rdf:type owl:NamedIndividual ,
                         :MessageTypeSet ;
                rdfs:isDefinedBy <https://w3id.org/won/auth#> .


###  https://w3id.org/won/auth#nodeSignedPropertyShape
:nodeSignedPropertyShape rdf:type owl:NamedIndividual ,
                                  <http://www.w3.org/ns/shacl#PropertyShape> ;
                         rdfs:isDefinedBy <https://w3id.org/won/auth#> ;
                         <http://www.w3.org/ns/shacl#datatype> xsd:boolean ;
                         <http://www.w3.org/ns/shacl#maxCount> 1 ;
                         <http://www.w3.org/ns/shacl#minCount> 0 ;
                         <http://www.w3.org/ns/shacl#nodeKind> <http://www.w3.org/ns/shacl#Literal> ;
                         <http://www.w3.org/ns/shacl#path> :nodeSigned .


###  https://w3id.org/won/auth#opAutoConnect
:opAutoConnect rdf:type owl:NamedIndividual ,
                        :SimpleOperationExpression ;
               rdfs:isDefinedBy <https://w3id.org/won/auth#> .


###  https://w3id.org/won/auth#opCommunicate
:opCommunicate rdf:type owl:NamedIndividual ,
                        :MessageOperationExpression ;
               :messageTo :msgTypesCommunicate ;
               rdfs:isDefinedBy <https://w3id.org/won/auth#> .


###  https://w3id.org/won/auth#opCommunicateOnBehalf
:opCommunicateOnBehalf rdf:type owl:NamedIndividual ,
                                :MessageOperationExpression ;
                       :messageOnBehalf :msgTypesCommunicate ;
                       rdfs:isDefinedBy <https://w3id.org/won/auth#> .


###  https://w3id.org/won/auth#opConnectAndCommunicateOnBehalf
:opConnectAndCommunicateOnBehalf rdf:type owl:NamedIndividual ,
                                          :MessageOperationExpression ;
                                 :messageOnBehalf :msgTypesCommunicate ,
                                                  :msgTypesConnectClose ;
                                 rdfs:isDefinedBy <https://w3id.org/won/auth#> .


###  https://w3id.org/won/auth#opConnectClose
:opConnectClose rdf:type owl:NamedIndividual ,
                         :MessageOperationExpression ;
                :messageTo :msgTypesConnectClose ;
                rdfs:isDefinedBy <https://w3id.org/won/auth#> .


###  https://w3id.org/won/auth#opConnectCloseOnBehalf
:opConnectCloseOnBehalf rdf:type owl:NamedIndividual ,
                                 :MessageOperationExpression ;
                        :messageOnBehalf :msgTypesConnectClose ;
                        rdfs:isDefinedBy <https://w3id.org/won/auth#> .


###  https://w3id.org/won/auth#opHint
:opHint rdf:type owl:NamedIndividual ,
                 :MessageOperationExpression ;
        :messageTo :msgTypesHint ;
        rdfs:isDefinedBy <https://w3id.org/won/auth#> .


###  https://w3id.org/won/auth#opModifyOnBehalf
:opModifyOnBehalf rdf:type owl:NamedIndividual ,
                           :MessageOperationExpression ;
                  :messageOnBehalf :msgTypesModify ;
                  rdfs:isDefinedBy <https://w3id.org/won/auth#> .


###  https://w3id.org/won/auth#opNop
:opNop rdf:type owl:NamedIndividual ,
                :SimpleOperationExpression ;
       rdfs:isDefinedBy <https://w3id.org/won/auth#> .


###  https://w3id.org/won/auth#opObserve
:opObserve rdf:type owl:NamedIndividual ,
                    :SimpleOperationExpression ;
           rdfs:isDefinedBy <https://w3id.org/won/auth#> .


###  https://w3id.org/won/auth#opRead
:opRead rdf:type owl:NamedIndividual ,
                 :SimpleOperationExpression ;
        rdfs:isDefinedBy <https://w3id.org/won/auth#> .


###  https://w3id.org/won/auth#operationPropertyShape
:operationPropertyShape rdf:type owl:NamedIndividual ,
                                 <http://www.w3.org/ns/shacl#PropertyShape> ;
                        rdfs:isDefinedBy <https://w3id.org/won/auth#> ;
                        <http://www.w3.org/ns/shacl#minCount> 1 ;
                        <http://www.w3.org/ns/shacl#or> [ ] ;
<http://www.w3.org/ns/shacl#path> :operation .


###  https://w3id.org/won/auth#operationRequestShape
:operationRequestShape rdf:type owl:NamedIndividual ,
                                <http://www.w3.org/ns/shacl#NodeShape> ;
                       rdfs:isDefinedBy <https://w3id.org/won/auth#> ;
                       <http://www.w3.org/ns/shacl#closed> "true"^^xsd:boolean ;
                       <http://www.w3.org/ns/shacl#ignoredProperties> [ ] ;
<http://www.w3.org/ns/shacl#or> [ ] ;
<http://www.w3.org/ns/shacl#property> _:genid108 ,
                                      _:genid109 ,
                                      _:genid110 ,
                                      _:genid112 ,
                                      _:genid113 ,
                                      _:genid114 ,
                                      _:genid115 ,
                                      _:genid116 ,
                                      _:genid117 ,
                                      _:genid118 ,
                                      _:genid119 ,
                                      _:genid120 ,
                                      _:genid121 ,
                                      _:genid122 ,
                                      _:genid123 ;
<http://www.w3.org/ns/shacl#targetClass> :OperationRequest .

_:genid108 <http://www.w3.org/ns/shacl#maxCount> 1 ;
            <http://www.w3.org/ns/shacl#nodeKind> <http://www.w3.org/ns/shacl#IRI> ;
            <http://www.w3.org/ns/shacl#path> :requestor .

_:genid109 <http://www.w3.org/ns/shacl#maxCount> 1 ;
            <http://www.w3.org/ns/shacl#node> :asePositionShape ;
            <http://www.w3.org/ns/shacl#path> :reqPosition .

_:genid110 <http://www.w3.org/ns/shacl#maxCount> 1 ;
            <http://www.w3.org/ns/shacl#or> [ ] ;
<http://www.w3.org/ns/shacl#path> :operation .

_:genid112 <http://www.w3.org/ns/shacl#maxCount> 1 ;
            <http://www.w3.org/ns/shacl#nodeKind> <http://www.w3.org/ns/shacl#IRI> ;
            <http://www.w3.org/ns/shacl#path> :reqAtom .

_:genid113 <http://www.w3.org/ns/shacl#node> :tokenSpecificationShape ;
            <http://www.w3.org/ns/shacl#path> :requestToken .

_:genid114 <http://www.w3.org/ns/shacl#maxCount> 1 ;
            <http://www.w3.org/ns/shacl#node> :atomStateShape ;
            <http://www.w3.org/ns/shacl#path> :reqAtomState .

_:genid115 <http://www.w3.org/ns/shacl#nodeKind> <http://www.w3.org/ns/shacl#IRI> ;
            <http://www.w3.org/ns/shacl#path> :reqGraph .

_:genid116 <http://www.w3.org/ns/shacl#node> :graphTypeShape ;
            <http://www.w3.org/ns/shacl#nodeKind> <http://www.w3.org/ns/shacl#IRI> ;
            <http://www.w3.org/ns/shacl#path> :reqGraphType .

_:genid117 <http://www.w3.org/ns/shacl#maxCount> 1 ;
            <http://www.w3.org/ns/shacl#nodeKind> <http://www.w3.org/ns/shacl#IRI> ;
            <http://www.w3.org/ns/shacl#path> :reqSocketType .

_:genid118 <http://www.w3.org/ns/shacl#maxCount> 1 ;
            <http://www.w3.org/ns/shacl#nodeKind> <http://www.w3.org/ns/shacl#IRI> ;
            <http://www.w3.org/ns/shacl#path> :reqSocket .

_:genid119 <http://www.w3.org/ns/shacl#maxCount> 1 ;
            <http://www.w3.org/ns/shacl#nodeKind> <http://www.w3.org/ns/shacl#IRI> ;
            <http://www.w3.org/ns/shacl#path> :reqConnection .

_:genid120 <http://www.w3.org/ns/shacl#maxCount> 1 ;
            <http://www.w3.org/ns/shacl#node> :connectionStateShape ;
            <http://www.w3.org/ns/shacl#path> :reqConnectionState .

_:genid121 <http://www.w3.org/ns/shacl#maxCount> 1 ;
            <http://www.w3.org/ns/shacl#nodeKind> <http://www.w3.org/ns/shacl#IRI> ;
            <http://www.w3.org/ns/shacl#path> :reqConnectionTargetAtom .

_:genid122 <http://www.w3.org/ns/shacl#maxCount> 1 ;
            <http://www.w3.org/ns/shacl#nodeKind> <http://www.w3.org/ns/shacl#IRI> ;
            <http://www.w3.org/ns/shacl#path> :reqConnectionMessage .

_:genid123 <http://www.w3.org/ns/shacl#node> :authTokenShape ;
            <http://www.w3.org/ns/shacl#path> :bearsToken .


###  https://w3id.org/won/auth#operationRequestor
:operationRequestor rdf:type owl:NamedIndividual ,
                             :RelativeAtomExpression ;
                    rdfs:isDefinedBy <https://w3id.org/won/auth#> .


###  https://w3id.org/won/auth#positionAtomGraph
:positionAtomGraph rdf:type owl:NamedIndividual ,
                            :AsePosition ;
                   rdfs:comment "Identifies the position of the __atom graph__ in the atom's tree structure"@en ;
                   rdfs:isDefinedBy <https://w3id.org/won/auth#> ;
                   :label "positionAtomGraph" ;
                   :parentPosition :positionRoot .


###  https://w3id.org/won/auth#positionAtomMessage
:positionAtomMessage rdf:type owl:NamedIndividual ,
                              :AsePosition ;
                     rdfs:comment "Identifies the position of the __atom message__ in the atom's tree structure"@en ;
                     rdfs:isDefinedBy <https://w3id.org/won/auth#> ;
                     :label "positionAtomMessage" ;
                     :parentPosition :positionAtomMessages .


###  https://w3id.org/won/auth#positionAtomMessages
:positionAtomMessages rdf:type owl:NamedIndividual ,
                               :AsePosition ;
                      rdfs:comment "Identifies the position of the __atom message container__ in the atom's tree structure"@en ;
                      rdfs:isDefinedBy <https://w3id.org/won/auth#> ;
                      :label "positionAtomMessages" ;
                      :parentPosition :positionRoot .


###  https://w3id.org/won/auth#positionConnection
:positionConnection rdf:type owl:NamedIndividual ,
                             :AsePosition ;
                    rdfs:comment "Identifies the position of the __connection__ in the atom's tree structure"@en ;
                    rdfs:isDefinedBy <https://w3id.org/won/auth#> ;
                    :label "positionConnection" ;
                    :parentPosition :positionConnections .


###  https://w3id.org/won/auth#positionConnectionMessage
:positionConnectionMessage rdf:type owl:NamedIndividual ,
                                    :AsePosition ;
                           rdfs:comment "Identifies the position of the __connection message__ in the atom's tree structure"@en ;
                           rdfs:isDefinedBy <https://w3id.org/won/auth#> ;
                           :label "positionConnectionMessage" ;
                           :parentPosition :positionConnectionMessages .


###  https://w3id.org/won/auth#positionConnectionMessages
:positionConnectionMessages rdf:type owl:NamedIndividual ,
                                     :AsePosition ;
                            rdfs:comment "Identifies the position of __connection message container__ in the atom's tree structure"@en ;
                            rdfs:isDefinedBy <https://w3id.org/won/auth#> ;
                            :label "positionConnectionMessages" ;
                            :parentPosition :positionConnection .


###  https://w3id.org/won/auth#positionConnections
:positionConnections rdf:type owl:NamedIndividual ,
                              :AsePosition ;
                     rdfs:comment "Identifies the position of the __connection container__ in the atom's tree structure"@en ;
                     rdfs:isDefinedBy <https://w3id.org/won/auth#> ;
                     :label "positionConnections" ;
                     :parentPosition :positionSocket .


###  https://w3id.org/won/auth#positionRoot
:positionRoot rdf:type owl:NamedIndividual ,
                       :AsePosition ;
              rdfs:comment "Identifies the root of the atom's tree structure"@en ;
              rdfs:isDefinedBy <https://w3id.org/won/auth#> ;
              :label "positionRoot" .


###  https://w3id.org/won/auth#positionSocket
:positionSocket rdf:type owl:NamedIndividual ,
                         :AsePosition ;
                rdfs:comment "Identifies the position of the __socket__ in the atom's tree structure"@en ;
                rdfs:isDefinedBy <https://w3id.org/won/auth#> ;
                :label "positionSocket" ;
                :parentPosition :positionRoot .


###  https://w3id.org/won/auth#relativeAtomExpressionShape
:relativeAtomExpressionShape rdf:type owl:NamedIndividual ,
                                      <http://www.w3.org/ns/shacl#NodeShape> ;
                             rdfs:isDefinedBy <https://w3id.org/won/auth#> ;
                             <http://www.w3.org/ns/shacl#closed> "true"^^xsd:boolean ;
                             <http://www.w3.org/ns/shacl#ignoredProperties> [ ] ;
<http://www.w3.org/ns/shacl#in> [ ] ;
<http://www.w3.org/ns/shacl#nodeKind> <http://www.w3.org/ns/shacl#IRI> .


###  https://w3id.org/won/auth#self
:self rdf:type owl:NamedIndividual ,
               :RelativeAtomExpression ;
      rdfs:isDefinedBy <https://w3id.org/won/auth#> .


###  https://w3id.org/won/auth#simpleOperationExpressionShape
:simpleOperationExpressionShape rdf:type owl:NamedIndividual ,
                                         <http://www.w3.org/ns/shacl#NodeShape> ,
                                         :OperationExpressionShape ;
                                rdfs:isDefinedBy <https://w3id.org/won/auth#> ;
                                <http://www.w3.org/ns/shacl#class> :SimpleOperationExpression ;
                                <http://www.w3.org/ns/shacl#closed> "true"^^xsd:boolean ;
                                <http://www.w3.org/ns/shacl#ignoredProperties> [ ] ;
<http://www.w3.org/ns/shacl#targetClass> :SimpleOperationExpression .


###  https://w3id.org/won/auth#socketExpressionShape
:socketExpressionShape rdf:type owl:NamedIndividual ,
                                <http://www.w3.org/ns/shacl#NodeShape> ,
                                :InheritingShape ,
                                :OperationContainerShape ,
                                :TargetAtomContainerShape ,
                                :TreeExpressionShape ;
                       rdfs:isDefinedBy <https://w3id.org/won/auth#> ;
                       <http://www.w3.org/ns/shacl#closed> "true"^^xsd:boolean ;
                       <http://www.w3.org/ns/shacl#ignoredProperties> [ ] ;
<http://www.w3.org/ns/shacl#or> [ ] ;
<http://www.w3.org/ns/shacl#targetObjectsOf> :socket ;
:asePosition :positionSocket .


###  https://w3id.org/won/auth#socketPropertyShape
:socketPropertyShape rdf:type owl:NamedIndividual ,
                              <http://www.w3.org/ns/shacl#PropertyShape> ;
                     rdfs:isDefinedBy <https://w3id.org/won/auth#> ;
                     <http://www.w3.org/ns/shacl#minCount> 1 ;
                     <http://www.w3.org/ns/shacl#node> :socketExpressionShape ;
                     <http://www.w3.org/ns/shacl#path> :socket .


###  https://w3id.org/won/auth#sysinfoGraph
:sysinfoGraph rdf:type owl:NamedIndividual ,
                       :GraphType ;
              rdfs:isDefinedBy <https://w3id.org/won/auth#> .


###  https://w3id.org/won/auth#targetAtomExpressionShape
:targetAtomExpressionShape rdf:type owl:NamedIndividual ,
                                    <http://www.w3.org/ns/shacl#NodeShape> ;
                           rdfs:isDefinedBy <https://w3id.org/won/auth#> ;
                           <http://www.w3.org/ns/shacl#closed> "true"^^xsd:boolean ;
                           <http://www.w3.org/ns/shacl#ignoredProperties> [ ] ;
<http://www.w3.org/ns/shacl#or> [ ] ;
<http://www.w3.org/ns/shacl#targetObjectsOf> :targetAtom .


###  https://w3id.org/won/auth#targetAtomPropertyShape
:targetAtomPropertyShape rdf:type owl:NamedIndividual ,
                                  <http://www.w3.org/ns/shacl#PropertyShape> ;
                         rdfs:isDefinedBy <https://w3id.org/won/auth#> ;
                         <http://www.w3.org/ns/shacl#maxCount> 1 ;
                         <http://www.w3.org/ns/shacl#minCount> 1 ;
                         <http://www.w3.org/ns/shacl#node> :targetAtomExpressionShape ;
                         <http://www.w3.org/ns/shacl#path> :targetAtom .


###  https://w3id.org/won/auth#targetAuthPropertyShape
:targetAuthPropertyShape rdf:type owl:NamedIndividual ,
                                  <http://www.w3.org/ns/shacl#PropertyShape> ;
                         rdfs:isDefinedBy <https://w3id.org/won/auth#> ;
                         <http://www.w3.org/ns/shacl#node> :authorizationShape ;
                         <http://www.w3.org/ns/shacl#path> :targetAuth .


###  https://w3id.org/won/auth#tokenExpPropertyShape
:tokenExpPropertyShape rdf:type owl:NamedIndividual ,
                                <http://www.w3.org/ns/shacl#PropertyShape> ;
                       rdfs:isDefinedBy <https://w3id.org/won/auth#> ;
                       <http://www.w3.org/ns/shacl#datatype> xsd:dateTime ;
                       <http://www.w3.org/ns/shacl#maxCount> 1 ;
                       <http://www.w3.org/ns/shacl#minCount> 1 ;
                       <http://www.w3.org/ns/shacl#nodeKind> <http://www.w3.org/ns/shacl#Literal> ;
                       <http://www.w3.org/ns/shacl#path> :tokenExp .


###  https://w3id.org/won/auth#tokenIatPropertyShape
:tokenIatPropertyShape rdf:type owl:NamedIndividual ,
                                <http://www.w3.org/ns/shacl#PropertyShape> ;
                       rdfs:isDefinedBy <https://w3id.org/won/auth#> ;
                       <http://www.w3.org/ns/shacl#datatype> xsd:dateTime ;
                       <http://www.w3.org/ns/shacl#maxCount> 1 ;
                       <http://www.w3.org/ns/shacl#minCount> 1 ;
                       <http://www.w3.org/ns/shacl#nodeKind> <http://www.w3.org/ns/shacl#Literal> ;
                       <http://www.w3.org/ns/shacl#path> :tokenIat .


###  https://w3id.org/won/auth#tokenIssPropertyShape
:tokenIssPropertyShape rdf:type owl:NamedIndividual ,
                                <http://www.w3.org/ns/shacl#PropertyShape> ;
                       rdfs:isDefinedBy <https://w3id.org/won/auth#> ;
                       <http://www.w3.org/ns/shacl#maxCount> 1 ;
                       <http://www.w3.org/ns/shacl#minCount> 1 ;
                       <http://www.w3.org/ns/shacl#nodeKind> <http://www.w3.org/ns/shacl#IRI> ;
                       <http://www.w3.org/ns/shacl#path> :tokenIss .


###  https://w3id.org/won/auth#tokenOperationExpressionShape
:tokenOperationExpressionShape rdf:type owl:NamedIndividual ,
                                        <http://www.w3.org/ns/shacl#NodeShape> ,
                                        :OperationExpressionShape ;
                               rdfs:isDefinedBy <https://w3id.org/won/auth#> ;
                               <http://www.w3.org/ns/shacl#closed> "true"^^xsd:boolean ;
                               <http://www.w3.org/ns/shacl#ignoredProperties> [ ] ;
<http://www.w3.org/ns/shacl#property> _:genid132 .

_:genid132 <http://www.w3.org/ns/shacl#maxCount> 1 ;
            <http://www.w3.org/ns/shacl#minCount> 1 ;
            <http://www.w3.org/ns/shacl#node> :tokenSpecificationShape ;
            <http://www.w3.org/ns/shacl#path> :requestToken .


###  https://w3id.org/won/auth#tokenScopePropertyShape
:tokenScopePropertyShape rdf:type owl:NamedIndividual ,
                                  <http://www.w3.org/ns/shacl#PropertyShape> ;
                         rdfs:isDefinedBy <https://w3id.org/won/auth#> ;
                         <http://www.w3.org/ns/shacl#maxCount> 1 ;
                         <http://www.w3.org/ns/shacl#minCount> 1 ;
                         <http://www.w3.org/ns/shacl#or> [ ] ;
<http://www.w3.org/ns/shacl#path> :tokenScope .


###  https://w3id.org/won/auth#tokenShapeShape
:tokenShapeShape rdf:type owl:NamedIndividual ,
                          <http://www.w3.org/ns/shacl#NodeShape> ;
                 rdfs:isDefinedBy <https://w3id.org/won/auth#> ;
                 <http://www.w3.org/ns/shacl#closed> "true"^^xsd:boolean ;
                 <http://www.w3.org/ns/shacl#property> :nodeSignedPropertyShape ,
                                                       _:genid134 ,
                                                       _:genid136 ;
                 <http://www.w3.org/ns/shacl#targetObjectsOf> :bearer .

_:genid134 <http://www.w3.org/ns/shacl#minCount> 1 ;
            <http://www.w3.org/ns/shacl#or> [ ] ;
<http://www.w3.org/ns/shacl#path> :tokenScope .

_:genid136 <http://www.w3.org/ns/shacl#minCount> 1 ;
            <http://www.w3.org/ns/shacl#or> [ ] ;
<http://www.w3.org/ns/shacl#path> :issuer .


###  https://w3id.org/won/auth#tokenSigPropertyShape
:tokenSigPropertyShape rdf:type owl:NamedIndividual ,
                                <http://www.w3.org/ns/shacl#PropertyShape> ;
                       rdfs:isDefinedBy <https://w3id.org/won/auth#> ;
                       <http://www.w3.org/ns/shacl#maxCount> 1 ;
                       <http://www.w3.org/ns/shacl#minCount> 0 ;
                       <http://www.w3.org/ns/shacl#nodeKind> <http://www.w3.org/ns/shacl#IRI> ;
                       <http://www.w3.org/ns/shacl#path> :tokenSig .


###  https://w3id.org/won/auth#tokenSpecificationShape
:tokenSpecificationShape rdf:type owl:NamedIndividual ,
                                  <http://www.w3.org/ns/shacl#NodeShape> ;
                         rdfs:isDefinedBy <https://w3id.org/won/auth#> ;
                         <http://www.w3.org/ns/shacl#closed> "true"^^xsd:boolean ;
                         <http://www.w3.org/ns/shacl#property> :expiresAfterPropertyShape ,
                                                               :nodeSignedPropertyShape ,
                                                               :tokenScopePropertyShape .


###  https://w3id.org/won/auth#tokenSubPropertyShape
:tokenSubPropertyShape rdf:type owl:NamedIndividual ,
                                <http://www.w3.org/ns/shacl#PropertyShape> ;
                       rdfs:isDefinedBy <https://w3id.org/won/auth#> ;
                       <http://www.w3.org/ns/shacl#maxCount> 1 ;
                       <http://www.w3.org/ns/shacl#minCount> 1 ;
                       <http://www.w3.org/ns/shacl#nodeKind> <http://www.w3.org/ns/shacl#IRI> ;
                       <http://www.w3.org/ns/shacl#path> :tokenSub .


[ <http://www.w3.org/ns/shacl#node> :simpleOperationExpressionShape
] .

[ <http://www.w3.org/ns/shacl#property> _:genid140
 ] .

_:genid140 <http://www.w3.org/ns/shacl#maxCount> 1 ;
            <http://www.w3.org/ns/shacl#minCount> 1 ;
            <http://www.w3.org/ns/shacl#node> :aseRootShape ;
            <http://www.w3.org/ns/shacl#path> :provideAuthInfo .

[ <http://www.w3.org/ns/shacl#nodeKind> <http://www.w3.org/ns/shacl#BlankNode>
 ] .

[ <http://www.w3.org/ns/shacl#node> :atomExpressionShape
 ] .

[ <http://www.w3.org/ns/shacl#property> _:genid144
 ] .

_:genid144 <http://www.w3.org/ns/shacl#minCount> 1 ;
            <http://www.w3.org/ns/shacl#node> :aseRootShape ;
            <http://www.w3.org/ns/shacl#path> :grantee .

[ <http://www.w3.org/ns/shacl#property> :connectionMessagesPropertyShape
 ] .

[ <http://www.w3.org/ns/shacl#datatype> xsd:integer
 ] .

[ <http://www.w3.org/ns/shacl#node> :tokenOperationExpressionShape
 ] .

[ <http://www.w3.org/ns/shacl#node> :messageOperationExpressionShape
 ] .

[ <http://www.w3.org/ns/shacl#property> :connectionMessagePropertyShape
 ] .

[ <http://www.w3.org/ns/shacl#property> _:genid151
 ] .

_:genid151 <http://www.w3.org/ns/shacl#maxCount> 1 ;
            <http://www.w3.org/ns/shacl#minCount> 1 ;
            <http://www.w3.org/ns/shacl#node> :granteeWildcardShape ;
            <http://www.w3.org/ns/shacl#path> :grantee .

[ <http://www.w3.org/ns/shacl#property> :targetAtomPropertyShape
 ] .

[ <http://www.w3.org/ns/shacl#property> _:genid154
 ] .

_:genid154 <http://www.w3.org/ns/shacl#minCount> 1 ;
            <http://www.w3.org/ns/shacl#node> :tokenShapeShape ;
            <http://www.w3.org/ns/shacl#path> :bearer .

[ <http://www.w3.org/ns/shacl#property> :operationPropertyShape
 ] .

[ <http://www.w3.org/ns/shacl#property> _:genid157
 ] .

_:genid157 <http://www.w3.org/ns/shacl#minCount> 1 ;
            <http://www.w3.org/ns/shacl#node> :aseRootShape ;
            <http://www.w3.org/ns/shacl#path> :grant .

[ <http://www.w3.org/ns/shacl#property> :operationPropertyShape
 ] .

[ <http://www.w3.org/ns/shacl#node> :relativeAtomExpressionShape
 ] .

[ <http://www.w3.org/ns/shacl#nodeKind> <http://www.w3.org/ns/shacl#IRI>
 ] .

[ <http://www.w3.org/ns/shacl#property> :inheritPropertyShape
 ] .

[ <http://www.w3.org/ns/shacl#property> _:genid163
 ] .

_:genid163 <http://www.w3.org/ns/shacl#node> :connectionMessageExpressionShape ;
            <http://www.w3.org/ns/shacl#path> :connectionMessage .

[ <http://www.w3.org/ns/shacl#property> :operationPropertyShape
 ] .

[ <http://www.w3.org/ns/shacl#property> :inheritPropertyShape
 ] .

[ <http://www.w3.org/ns/shacl#property> :targetAtomPropertyShape
 ] .

[ <http://www.w3.org/ns/shacl#property> :operationPropertyShape
 ] .

[ <http://www.w3.org/ns/shacl#property> :inheritPropertyShape
 ] .

[ <http://www.w3.org/ns/shacl#property> _:genid170
 ] .

_:genid170 <http://www.w3.org/ns/shacl#node> :connectionStateShape ;
            <http://www.w3.org/ns/shacl#path> :connectionState .

[ <http://www.w3.org/ns/shacl#property> :connectionPropertyShape
 ] .

[ <http://www.w3.org/ns/shacl#property> :connectionMessagesPropertyShape
 ] .

[ <http://www.w3.org/ns/shacl#property> :connectionMessagePropertyShape
 ] .

[ <http://www.w3.org/ns/shacl#property> :targetAtomPropertyShape
 ] .

[ <http://www.w3.org/ns/shacl#property> :atomMessagePropertyShape
 ] .

[ <http://www.w3.org/ns/shacl#property> :inheritPropertyShape
 ] .

[ <http://www.w3.org/ns/shacl#property> :inheritPropertyShape
 ] .

[ <http://www.w3.org/ns/shacl#property> :operationPropertyShape
 ] .

[ <http://www.w3.org/ns/shacl#property> :operationPropertyShape
 ] .

[ <http://www.w3.org/ns/shacl#property> :inheritPropertyShape
 ] .

[ <http://www.w3.org/ns/shacl#property> _:genid182
 ] .

_:genid182 <http://www.w3.org/ns/shacl#node> :graphTypeShape ;
            <http://www.w3.org/ns/shacl#path> :graphType .

[ <http://www.w3.org/ns/shacl#property> :operationPropertyShape
 ] .

[ <http://www.w3.org/ns/shacl#property> :inheritPropertyShape
 ] .

[ <http://www.w3.org/ns/shacl#property> _:genid186
 ] .

_:genid186 <http://www.w3.org/ns/shacl#minCount> 1 ;
            <http://www.w3.org/ns/shacl#node> :atomExpressionShape ;
            <http://www.w3.org/ns/shacl#path> :grantee .

[ <http://www.w3.org/ns/shacl#property> _:genid188
 ] .

_:genid188 <http://www.w3.org/ns/shacl#node> :connectionStateShape ;
            <http://www.w3.org/ns/shacl#path> :connectionState .

[ <http://www.w3.org/ns/shacl#property> :connectionPropertyShape
 ] .

[ <http://www.w3.org/ns/shacl#nodeKind> <http://www.w3.org/ns/shacl#IRI>
 ] .

[ <http://www.w3.org/ns/shacl#property> :connectionMessagesPropertyShape
 ] .

[ <http://www.w3.org/ns/shacl#property> _:genid193
 ] .

_:genid193 <http://www.w3.org/ns/shacl#nodeKind> <http://www.w3.org/ns/shacl#IRI> ;
            <http://www.w3.org/ns/shacl#path> :graphIri .

[ <http://www.w3.org/ns/shacl#property> :operationPropertyShape
 ] .

_:genid195 <http://www.w3.org/ns/shacl#datatype> xsd:string ;
            <http://www.w3.org/ns/shacl#nodeKind> <http://www.w3.org/ns/shacl#Literal> ;
            <http://www.w3.org/ns/shacl#pattern> "^[^\\s]+$" .

[ <http://www.w3.org/ns/shacl#property> :connectionMessagePropertyShape
 ] .

[ <http://www.w3.org/ns/shacl#node> :atomExpressionShape
 ] .

[ <http://www.w3.org/ns/shacl#property> :targetAtomPropertyShape
 ] .

[ <http://www.w3.org/ns/shacl#node> :aseRootShape
 ] .

[ <http://www.w3.org/ns/shacl#property> :operationPropertyShape
 ] .

[ <http://www.w3.org/ns/shacl#node> :simpleOperationExpressionShape
 ] .

_:genid202 <http://www.w3.org/ns/shacl#datatype> xsd:string ;
            <http://www.w3.org/ns/shacl#nodeKind> <http://www.w3.org/ns/shacl#Literal> ;
            <http://www.w3.org/ns/shacl#pattern> "^[^\\s]+$" .

[ <http://www.w3.org/ns/shacl#node> :messageOperationExpressionShape
 ] .

[ <http://www.w3.org/ns/shacl#node> :tokenOperationExpressionShape
 ] .

[ <http://www.w3.org/ns/shacl#datatype> xsd:long
 ] .

[ <http://www.w3.org/ns/shacl#datatype> xsd:int
 ] .

[ <http://www.w3.org/ns/shacl#nodeKind> <http://www.w3.org/ns/shacl#IRI>
 ] .

_:genid208 <http://www.w3.org/ns/shacl#minCount> 1 ;
            <http://www.w3.org/ns/shacl#path> :requestor .

_:genid209 <http://www.w3.org/ns/shacl#minCount> 1 ;
            <http://www.w3.org/ns/shacl#path> :bearsToken .

[ <http://www.w3.org/ns/shacl#property> :inheritPropertyShape
 ] .

[ <http://www.w3.org/ns/shacl#property> :atomMessagePropertyShape
 ] .

[ <http://www.w3.org/ns/shacl#property> _:genid213
 ] .

_:genid213 <http://www.w3.org/ns/shacl#node> :aseRootShape ;
            <http://www.w3.org/ns/shacl#path> :grantee .

[ <http://www.w3.org/ns/shacl#node> :messageTypesExpressionShape
 ] .

[ <http://www.w3.org/ns/shacl#property> _:genid216
 ] .

_:genid216 <http://www.w3.org/ns/shacl#nodeKind> <http://www.w3.org/ns/shacl#IRI> ;
            <http://www.w3.org/ns/shacl#path> :socketType .

[ <http://www.w3.org/ns/shacl#node> :messageTypeShape
 ] .

[ <http://www.w3.org/ns/shacl#property> _:genid219
 ] .

_:genid219 <http://www.w3.org/ns/shacl#maxCount> 1 ;
            <http://www.w3.org/ns/shacl#node> :granteeWildcardShape ;
            <http://www.w3.org/ns/shacl#path> :grantee .

[ <http://www.w3.org/ns/shacl#property> _:genid221
 ] .

_:genid221 <http://www.w3.org/ns/shacl#maxCount> 1 ;
            <http://www.w3.org/ns/shacl#minCount> 1 ;
            <http://www.w3.org/ns/shacl#node> :messageWildcardShape ;
            <http://www.w3.org/ns/shacl#path> :messageOnBehalf .

[ <http://www.w3.org/ns/shacl#property> _:genid223
 ] .

_:genid223 <http://www.w3.org/ns/shacl#nodeKind> <http://www.w3.org/ns/shacl#IRI> ;
            <http://www.w3.org/ns/shacl#path> :socketIri .

[ <http://www.w3.org/ns/shacl#property> :atomStatePropertyShape
 ] .

[ <http://www.w3.org/ns/shacl#property> :graphPropertyShape
 ] .

[ <http://www.w3.org/ns/shacl#property> :atomMessagesPropertyShape
 ] .

[ <http://www.w3.org/ns/shacl#property> :connectionsPropertyShape
 ] .

[ <http://www.w3.org/ns/shacl#property> _:genid229
 ] .

_:genid229 <http://www.w3.org/ns/shacl#minCount> 1 ;
            <http://www.w3.org/ns/shacl#or> [ ] ;
<http://www.w3.org/ns/shacl#path> :messageTo .

[ <http://www.w3.org/ns/shacl#node> :messageTypesExpressionShape
 ] .

[ <http://www.w3.org/ns/shacl#node> :messageTypeShape
 ] .

[ <http://www.w3.org/ns/shacl#property> _:genid234
 ] .

_:genid234 <http://www.w3.org/ns/shacl#maxCount> 1 ;
            <http://www.w3.org/ns/shacl#minCount> 1 ;
            <http://www.w3.org/ns/shacl#node> :messageWildcardShape ;
            <http://www.w3.org/ns/shacl#path> :messageTo .

[ <http://www.w3.org/ns/shacl#property> :connectionsPropertyShape
 ] .

[ <http://www.w3.org/ns/shacl#property> :connectionPropertyShape
 ] .

[ <http://www.w3.org/ns/shacl#property> :connectionMessagesPropertyShape
 ] .

[ <http://www.w3.org/ns/shacl#property> :connectionMessagePropertyShape
 ] .

[ <http://www.w3.org/ns/shacl#property> :socketPropertyShape
 ] .

[ <http://www.w3.org/ns/shacl#property> _:genid241
 ] .

_:genid241 <http://www.w3.org/ns/shacl#node> :tokenShapeShape ;
            <http://www.w3.org/ns/shacl#path> :bearer .

[ <http://www.w3.org/ns/shacl#property> _:genid243
 ] .

_:genid243 <http://www.w3.org/ns/shacl#minCount> 1 ;
            <http://www.w3.org/ns/shacl#or> [ ] ;
<http://www.w3.org/ns/shacl#path> :messageOnBehalf .

#################################################################
#    Annotations
#################################################################

:AseFilterProperty rdfs:comment "Object properties that can be used to filter the focus nodes of ASE expressions."@en ;
                    rdfs:isDefinedBy <https://w3id.org/won/auth#> ;
                    rdfs:label "AseFilterProperty" .


:AseLeafProperty rdfs:comment "Object properties of ASEs that do not have ASEs as their object."@en ;
                 rdfs:isDefinedBy <https://w3id.org/won/auth#> ;
                 rdfs:label "AseLeafProperty" .


:expiresAfter rdfs:comment "Specifies the lifetime of a token in seconds."@en ;
              rdfs:isDefinedBy <https://w3id.org/won/auth#> ;
              rdfs:label "expiresAfter" .


:inherit rdfs:comment """Atom structure expressions use `auth:inherit true` in order to not inherit granted operations from
        their parent expressions"""@en ;
         rdfs:isDefinedBy <https://w3id.org/won/auth#> ;
         rdfs:label "inherit" .


:operation rdfs:comment """Used in ASEs to enumerate operations granted for the ASE's position in the atom's tree structure.
        When checking for granted operations, operations are inherited by nested ASEs. An ASE can reject inheriting
        the granted operations using `auth:inherit false`."""@en ;
           rdfs:isDefinedBy <https://w3id.org/won/auth#> ;
           rdfs:label "operation" .


:targetAtom rdfs:comment "Identifies target atoms of connections that are direct or transitive targetNodes of the expression's focus nodes."@en ;
            rdfs:isDefinedBy <https://w3id.org/won/auth#> ;
            rdfs:label "targetAtom" .


:tokenExp rdfs:comment "The date/time the token expires, according to the signer's clock."@en ;
          rdfs:isDefinedBy <https://w3id.org/won/auth#> ;
          rdfs:label "tokenExp" .


:tokenIat rdfs:comment "The date/time the token was issued, according to the signer's clock."@en ;
          rdfs:isDefinedBy <https://w3id.org/won/auth#> ;
          rdfs:label "tokenIat" .


:tokenScope rdfs:comment "Scope of an actual token, of a token to be granted, or required scope of a token to be accepted."@en ,
                         """The auth:tokenScope property is used to annotate which scope value a token has, is requested with, 
    or is required to have. Token scopes with URI values allow different socket definitions to collaborate: one socket
    adds an authorization to an atom granting a token with a specific scope URI, another socket specifies an authorization
    requiring a token with that scope URI (from a defined set of accepted issuers) in order to grant some operation."""@en ;
            rdfs:isDefinedBy <https://w3id.org/won/auth#> ;
            rdfs:label "tokenScope" .


###  Generated by the OWL API (version 5.1.9) https://github.com/owlcs/owlapi/
