@prefix : <https://w3id.org/won/ext/persona#> .
@prefix owl: <http://www.w3.org/2002/07/owl#> .
@prefix rdf: <http://www.w3.org/1999/02/22-rdf-syntax-ns#> .
@prefix xml: <http://www.w3.org/XML/1998/namespace> .
@prefix xsd: <http://www.w3.org/2001/XMLSchema#> .
@prefix rdfs: <http://www.w3.org/2000/01/rdf-schema#> .
@base <https://w3id.org/won/ext/persona> .

<https://w3id.org/won/ext/persona> rdf:type owl:Ontology ;
                                    owl:versionIRI <https://w3id.org/won/ext/persona/1.0> ;
                                    owl:imports <https://w3id.org/won/core> ;
                                    <http://purl.org/dc/elements/1.1/abstract> "This ontology contains the definition of the *InterestSocket* the *InterestOfSocket* the *ExpertiseSocket* and the *ExpertiseOfSocket*, the *interest* the *interestOf* the *expertise* and the *expertOf* properties. These express control relationships in WoN. The Atoms with expertise/interest in other atoms represent agents (users or programs) and can themselves not be interests/expertises of other atoms."@en ;
                                    <http://purl.org/dc/elements/1.1/creator> "Fabian Suda" ;
                                    <http://purl.org/dc/elements/1.1/date> "2021-02-02"^^xsd:date ;
                                    <http://purl.org/dc/elements/1.1/title> "Web of Needs Persona Extension" ;
                                    <http://purl.org/dc/terms/license> <https://creativecommons.org/licenses/by/4.0/> ;
                                    <http://purl.org/vocab/vann/preferredNamespacePrefix> "wx-persona" .

#################################################################
#    Annotation properties
#################################################################

###  http://purl.org/dc/elements/1.1/abstract
<http://purl.org/dc/elements/1.1/abstract> rdf:type owl:AnnotationProperty .


###  http://purl.org/dc/elements/1.1/creator
<http://purl.org/dc/elements/1.1/creator> rdf:type owl:AnnotationProperty .


###  http://purl.org/dc/elements/1.1/date
<http://purl.org/dc/elements/1.1/date> rdf:type owl:AnnotationProperty .


###  http://purl.org/dc/elements/1.1/description
<http://purl.org/dc/elements/1.1/description> rdf:type owl:AnnotationProperty .


###  http://purl.org/dc/elements/1.1/title
<http://purl.org/dc/elements/1.1/title> rdf:type owl:AnnotationProperty .


###  http://purl.org/dc/terms/license
<http://purl.org/dc/terms/license> rdf:type owl:AnnotationProperty .


###  http://purl.org/vocab/vann/preferredNamespacePrefix
<http://purl.org/vocab/vann/preferredNamespacePrefix> rdf:type owl:AnnotationProperty .


###  http://www.w3.org/2000/01/rdf-schema#labels
rdfs:labels rdf:type owl:AnnotationProperty .


#################################################################
#    Object Properties
#################################################################

###  https://w3id.org/won/ext/persona#expertise
:expertise rdf:type owl:ObjectProperty ;
           rdfs:domain <https://w3id.org/won/core#Atom> ;
           rdfs:range <https://w3id.org/won/core#Atom> ;
           owl:propertyDisjointWith :expertiseOf .


###  https://w3id.org/won/ext/persona#expertiseOf
:expertiseOf rdf:type owl:ObjectProperty ;
             rdfs:domain <https://w3id.org/won/core#Atom> ;
             rdfs:range <https://w3id.org/won/core#Atom> .


###  https://w3id.org/won/ext/persona#interest
:interest rdf:type owl:ObjectProperty ;
          rdfs:domain <https://w3id.org/won/core#Atom> ;
          rdfs:range <https://w3id.org/won/core#Atom> ;
          owl:propertyDisjointWith :interestOf .


###  https://w3id.org/won/ext/persona#interestOf
:interestOf rdf:type owl:ObjectProperty ;
            rdfs:domain <https://w3id.org/won/core#Atom> ;
            rdfs:range <https://w3id.org/won/core#Atom> .


#################################################################
#    Classes
#################################################################

###  https://w3id.org/won/ext/persona#Expertise
:Expertise rdf:type owl:Class ;
           rdfs:comment "Announce an expertise in something, such as a technology or framework."@en ;
           rdfs:label "Expertise" .


###  https://w3id.org/won/ext/persona#Interest
:Interest rdf:type owl:Class ;
          rdfs:comment "Announce an interest in something, such as a hobby."@en ;
          rdfs:label "Interest" .


#################################################################
#    Individuals
#################################################################

###  https://w3id.org/won/ext/persona#ExpertiseOfSocket
:ExpertiseOfSocket rdf:type owl:NamedIndividual ,
                            <https://w3id.org/won/core#SocketDefinition> ;
                   <https://w3id.org/won/core#compatibleSocketDefinition> :ExpertiseSocket ;
                   <https://w3id.org/won/core#derivesAtomProperty> :expertiseOf ;
                   <https://w3id.org/won/core#autoOpen> "false"^^xsd:boolean ;
                   <https://w3id.org/won/core#socketCapacity> 1 ;
                   rdfs:comment "An Atom uses a Socket with this configuration to identify an expertise of the Persona Atom that it is connected to"@en ;
                   rdfs:label "ExpertiseOfSocket" .


###  https://w3id.org/won/ext/persona#ExpertiseSocket
:ExpertiseSocket rdf:type owl:NamedIndividual ,
                          <https://w3id.org/won/core#SocketDefinition> ;
                 <https://w3id.org/won/core#compatibleSocketDefinition> :ExpertiseOfSocket ;
                 <https://w3id.org/won/core#derivesAtomProperty> :expertise ;
                 <https://w3id.org/won/core#autoOpen> "false"^^xsd:boolean ;
                 rdfs:comment "A Persona Atom uses a Socket with this configuration to represent Expertises."@en ;
                 rdfs:label "ExpertiseSocket" .


###  https://w3id.org/won/ext/persona#InterestOfSocket
:InterestOfSocket rdf:type owl:NamedIndividual ,
                           <https://w3id.org/won/core#SocketDefinition> ;
                  <https://w3id.org/won/core#compatibleSocketDefinition> :InterestSocket ;
                  <https://w3id.org/won/core#derivesAtomProperty> :interestOf ;
                  <https://w3id.org/won/core#autoOpen> "false"^^xsd:boolean ;
                  <https://w3id.org/won/core#socketCapacity> 1 ;
                  rdfs:comment "An Atom uses a Socket with this configuration to identify an interest of the Persona Atom that it is connected to."@en ;
                  rdfs:label "InterestOfSocket" .


###  https://w3id.org/won/ext/persona#InterestSocket
:InterestSocket rdf:type owl:NamedIndividual ,
                         <https://w3id.org/won/core#SocketDefinition> ;
                <https://w3id.org/won/core#compatibleSocketDefinition> :InterestOfSocket ;
                <https://w3id.org/won/core#derivesAtomProperty> :interest ;
                <https://w3id.org/won/core#autoOpen> "false"^^xsd:boolean ;
                rdfs:comment "A Persona Atom uses a Socket with this configuration to represent Interests."@en ;
                rdfs:label "InterestSocket" .


###  https://w3id.org/won/ext/persona#expertise
:expertise rdf:type owl:NamedIndividual .


###  https://w3id.org/won/ext/persona#expertiseOf
:expertiseOf rdf:type owl:NamedIndividual .


###  https://w3id.org/won/ext/persona#interest
:interest rdf:type owl:NamedIndividual .


###  https://w3id.org/won/ext/persona#interestOf
:interestOf rdf:type owl:NamedIndividual .


#################################################################
#    Annotations
#################################################################

:expertise rdfs:comment "Links the Atom representing an agent (a person, organization, bot, ...) to another Atom they control."@en ;
           rdfs:label "expertise" .


:expertiseOf rdfs:comment "Links an Atom to the Atom representing the agent (a person, organization, bot, ...) that controls both."@en ;
             rdfs:label "expertiseOf" .


:interest rdfs:comment "Links the Atom representing an agent (a person, organization, bot, ...) to another Atom they control."@en ;
          rdfs:label "interest" .


:interestOf rdfs:comment "Links an Atom to the Atom representing the agent (a person, organization, bot, ...) that controls both."@en ;
            rdfs:label "interestOf" .


#################################################################
#    General axioms
#################################################################

[ rdf:type owl:AllDifferent ;
  owl:distinctMembers ( :ExpertiseOfSocket
                        :ExpertiseSocket
                        :InterestOfSocket
                        :InterestSocket
                      )
] .


###  Generated by the OWL API (version 5.1.14) https://github.com/owlcs/owlapi/
